Proved that int_trans_bf preserves the sat and dissat property.

Theory.v
@@ -4,8 +4,8 @@ Require Import FunctionalExtensionality.
 
 (* Abstract Variable Type *)
 Module Type VARIABLE.
-Parameter var        : Type.
-Parameter var_eq_dec : forall v1 v2 : var, {v1 = v2} + {v1 <> v2}.
+  Parameter var        : Type.
+  Parameter var_eq_dec : forall v1 v2 : var, {v1 = v2} + {v1 <> v2}.
 End VARIABLE.
 
 (* Semantic Value Type *)
@@ -22,6 +22,15 @@ Module Type SEM_VAL.
   Axiom truth_or_assoc : forall v1 v2 v3, truth_or v1 (truth_or v2 v3) = truth_or (truth_or v1 v2) v3.
   Axiom truth_or_true_iff : forall v1 v2, truth_or v1 v2 = bool_inj true <-> v1 = bool_inj true \/ v2 = bool_inj true.
   Axiom truth_and_true_iff : forall v1 v2, truth_and v1 v2 = bool_inj true <-> v1 = bool_inj true /\ v2 = bool_inj true.
+  Axiom tautology_1 : truth_not (bool_inj false) = (bool_inj true).
+  Axiom tautology_2 : truth_not (bool_inj true) = (bool_inj false).
+  Axiom tautology_3 : forall v, truth_and v v = v.
+  Axiom tautology_4 : truth_and (bool_inj true) (bool_inj false) = bool_inj false.
+  Axiom tautology_5 : truth_and (bool_inj false) (bool_inj true) = bool_inj false.
+  Axiom tautology_6 : forall v, truth_or v v = v.
+  Axiom tautology_7 : truth_or (bool_inj true) (bool_inj false) = bool_inj true.
+  Axiom tautology_8 : truth_or (bool_inj false) (bool_inj true) = bool_inj true.
+
 End SEM_VAL.
 
 Module Three_Val <: SEM_VAL.
@@ -85,6 +94,15 @@ Module Three_Val <: SEM_VAL.
   Lemma truth_and_true_iff : forall v1 v2, truth_and v1 v2 = bool_inj true <-> v1 = bool_inj true /\ v2 = bool_inj true.
   Proof. intros; destruct v1, v2; simpl; intuition; inversion H. Qed.
 
+  Lemma tautology_1 : truth_not (bool_inj false) = (bool_inj true). Proof. intuition. Qed.
+  Lemma tautology_2 : truth_not (bool_inj true) = (bool_inj false). Proof. intuition. Qed.
+  Lemma tautology_3 : forall v, truth_and v v = v. Proof. intros; destruct v; simpl; trivial. Qed.
+  Lemma tautology_4 : truth_and (bool_inj true) (bool_inj false) = bool_inj false. Proof. intuition. Qed.
+  Lemma tautology_5 : truth_and (bool_inj false) (bool_inj true) = bool_inj false. Proof. intuition. Qed.
+  Lemma tautology_6 : forall v, truth_or v v = v. Proof. intros; destruct v; simpl; trivial. Qed.
+  Lemma tautology_7 : truth_or (bool_inj true) (bool_inj false) = bool_inj true. Proof. intuition. Qed.
+  Lemma tautology_8 : truth_or (bool_inj false) (bool_inj true) = bool_inj true. Proof. intuition. Qed.
+
 End Three_Val.
 
 Module Bool_Val <: SEM_VAL.
@@ -113,6 +131,15 @@ Module Bool_Val <: SEM_VAL.
 
   Lemma truth_and_true_iff : forall v1 v2, truth_and v1 v2 = bool_inj true <-> v1 = bool_inj true /\ v2 = bool_inj true.
   Proof. intros; unfold bool_inj; simpl; apply andb_true_iff. Qed.
+
+  Lemma tautology_1 : truth_not (bool_inj false) = (bool_inj true). Proof. intuition. Qed.
+  Lemma tautology_2 : truth_not (bool_inj true) = (bool_inj false). Proof. intuition. Qed.
+  Lemma tautology_3 : forall v, truth_and v v = v. Proof. intros; destruct v; simpl; trivial. Qed.
+  Lemma tautology_4 : truth_and (bool_inj true) (bool_inj false) = bool_inj false. Proof. intuition. Qed.
+  Lemma tautology_5 : truth_and (bool_inj false) (bool_inj true) = bool_inj false. Proof. intuition. Qed.
+  Lemma tautology_6 : forall v, truth_or v v = v. Proof. intros; destruct v; simpl; trivial. Qed.
+  Lemma tautology_7 : truth_or (bool_inj true) (bool_inj false) = bool_inj true. Proof. intuition. Qed.
+  Lemma tautology_8 : truth_or (bool_inj false) (bool_inj true) = bool_inj true. Proof. intuition. Qed.
 
 End Bool_Val.
 
@@ -176,6 +203,117 @@ Module ZInfinity <: NUMBER.
       | Some (ZE_Fin z1), Some (ZE_Fin z2) => Some (ZE_Fin (z1 + z2))
     end.
 
+  (* If sum is finite, then both addend and augend are finite. *)
+  Lemma numplus_finite : forall v1 v2 z, num_plus v1 v2 = Some (ZE_Fin z)
+                                         -> exists z1 z2, (v1 = Some (ZE_Fin z1)) /\
+                                                          (v2 = Some (ZE_Fin z2)) /\
+                                                          (z1 + z2 = z)%Z.
+  Proof.
+    intros until z.
+    destruct v1, v2; intros; try discriminate H.
+    destruct z0, z1; try discriminate H.
+    exists z0, z1; simpl in *.
+    split; auto.
+    split; auto.
+    injection H; auto.
+    destruct z0; discriminate H.
+  Qed.
+
+  (* If negation is finite, then the original is finite. *)
+  Lemma numneg_finite : forall v z, num_neg v = Some (ZE_Fin z)
+                                    -> exists x, v = Some (ZE_Fin x) /\ (- x = z)%Z.
+  Proof.
+    intros until z.
+    destruct v; intros; try discriminate H.
+    destruct z0; try discriminate H.
+    exists z0.
+    split; auto.
+    simpl in H.
+    injection H.
+    auto.
+  Qed.
+
+  (* If sum is positive infinity, then at least one addend is positive
+  infinity and neither of them is negative infinity. *)
+  Lemma numplus_inf : forall v1 v2, num_plus v1 v2 = Some ZE_Inf
+                                    -> ((exists z, v1 = Some (ZE_Fin z)) /\ v2 = Some ZE_Inf) \/
+                                       (v1 = Some ZE_Inf /\ (exists z, v2 = Some (ZE_Fin z))) \/
+                                       (v1 = Some ZE_Inf /\ v2 = Some ZE_Inf).
+  Proof.
+    intros.
+    destruct v1, v2.
+    destruct z, z0; simpl in *; auto;
+    try (discriminate H).
+    left; split; auto; exists z; auto.
+    right; left; split; auto; exists z; auto.
+    simpl in H; destruct z; discriminate H.
+    simpl in H; destruct z; discriminate H.
+    simpl in H; discriminate H.
+  Qed.
+
+  (* If sum is negative infinity, then at least one addend is negative
+  infinity and neither of them is positive infinity. *)
+  Lemma numplus_neginf : forall v1 v2, num_plus v1 v2 = Some ZE_NegInf
+                                       -> ((exists z, v1 = Some (ZE_Fin z)) /\ v2 = Some ZE_NegInf) \/
+                                          (v1 = Some ZE_NegInf /\ (exists z, v2 = Some (ZE_Fin z))) \/
+                                          (v1 = Some ZE_NegInf /\ v2 = Some ZE_NegInf).
+  Proof.
+    intros.
+    destruct v1, v2.
+    destruct z, z0; simpl in *; auto;
+    try (discriminate H).
+    left; split; auto; exists z; auto.
+    right; left; split; auto; exists z; auto.
+    simpl in H; destruct z; discriminate H.
+    simpl in H; destruct z; discriminate H.
+    simpl in H; discriminate H.
+  Qed.
+
+  (* If negation is positive infinity, then the original is negative infinity. *)
+  Lemma numneg_inf : forall v, num_neg v = Some ZE_Inf
+                               -> v = Some (ZE_NegInf).
+  Proof.
+    destruct v; intros; try discriminate H.
+    destruct z; try discriminate H.
+    auto.
+  Qed.
+
+  (* If negation is negative infinity, then the original is positive infinity. *)
+  Lemma numneg_neginf : forall v, num_neg v = Some ZE_NegInf
+                                  -> v = Some (ZE_Inf).
+  Proof.
+    destruct v; intros; try discriminate H.
+    destruct z; try discriminate H.
+    auto.
+  Qed.
+
+  (* If sum has no definition, then either of addends has no
+  definition or it's the sum of positive infinity and negative
+  infinity. *)
+  Lemma numplus_none : forall v1 v2, num_plus v1 v2 = None -> v1 = None \/ v2 = None \/
+                                                              (v1 = Some ZE_Inf /\ v2 = Some ZE_NegInf) \/
+                                                              (v1 = Some ZE_NegInf /\ v2 = Some ZE_Inf).
+  Proof.
+    intros.
+    destruct v1, v2.
+    right; right.
+    destruct z, z0; try discriminate H.
+    left; auto.
+    right; auto.
+    right; left; auto.
+    left; auto.
+    left; auto.
+  Qed.
+
+  (* If the negation has no definition, then the original has no definition *)
+  Lemma numneg_none: forall v, num_neg v = None -> v = None.
+  Proof.
+    intros.
+    destruct v.
+    destruct z; simpl in H; discriminate H.
+    auto.
+  Qed.
+
 End ZInfinity.
 
 (* Normal Integer Number Field *)
@@ -200,29 +338,45 @@ Module FinLeqRelation (VAL : SEM_VAL) <: LEQ_RELATION ZNumLattice VAL.
 End FinLeqRelation.
 
 Module Type NONE_RELATION (VAL : SEM_VAL).
-  Import ZInfinity.
   Import VAL.
-  Parameter none_leq : A -> Val.
-  Parameter leq_none : A -> Val.
+  Parameter noneVal : Val.
+  Axiom none_tautology_1 : truth_and noneVal (truth_not noneVal) = noneVal.
+  Axiom none_tautology_2 : truth_and noneVal (bool_inj true) = noneVal.
+  Axiom none_tautology_3 : truth_and noneVal (bool_inj false) = bool_inj false.
+  Axiom none_tautology_4 : truth_or noneVal (bool_inj false) = noneVal.
+  Axiom none_tautology_5 : truth_or (bool_inj false) noneVal = noneVal.
 End NONE_RELATION.
 
 Module None3ValRel <: NONE_RELATION Three_Val.
-  Import ZInfinity Three_Val.
-  Definition none_leq := fun _ : A => VUnknown.
-  Definition leq_none := fun _ : A => VUnknown.
+  Import Three_Val.
+  Definition noneVal := VUnknown.
+  Lemma none_tautology_1 : truth_and noneVal (truth_not noneVal) = noneVal. Proof. intuition. Qed.
+  Lemma none_tautology_2 : truth_and noneVal (bool_inj true) = noneVal. Proof. intuition. Qed.
+  Lemma none_tautology_3 : truth_and noneVal (bool_inj false) = bool_inj false. Proof. intuition. Qed.
+  Lemma none_tautology_4 : truth_or noneVal (bool_inj false) = noneVal. Proof. intuition. Qed.
+  Lemma none_tautology_5 : truth_or (bool_inj false) noneVal = noneVal. Proof. intuition. Qed.
+
 End None3ValRel.
 
 Module NoneAlwaysFalse (VAL : SEM_VAL) <: NONE_RELATION VAL.
-  Import ZInfinity VAL.
-  Definition none_leq := fun _ : A => bool_inj false.
-  Definition leq_none := fun _ : A => bool_inj false.
-End NoneAlwaysFalse.
+  Import VAL.
+  Definition noneVal := bool_inj false.
+  Lemma none_tautology_1 : truth_and noneVal (truth_not noneVal) = noneVal.
+  Proof. unfold noneVal; simpl; rewrite tautology_1, tautology_5; trivial. Qed.
 
-Module NoneAlwaysTrue (VAL : SEM_VAL) <: NONE_RELATION VAL.
-  Import ZInfinity VAL.
-  Definition none_leq := fun _ : A => bool_inj true.
-  Definition leq_none := fun _ : A => bool_inj true.
-End NoneAlwaysTrue.
+  Lemma none_tautology_2 : truth_and noneVal (bool_inj true) = noneVal.
+  Proof. unfold noneVal; simpl; rewrite tautology_5; trivial. Qed.
+
+  Lemma none_tautology_3 : truth_and noneVal (bool_inj false) = bool_inj false.
+  Proof. unfold noneVal; simpl; rewrite tautology_3; trivial. Qed.
+
+  Lemma none_tautology_4 : truth_or noneVal (bool_inj false) = noneVal.
+  Proof. unfold noneVal; simpl; rewrite tautology_6; trivial. Qed.
+
+  Lemma none_tautology_5 : truth_or (bool_inj false) noneVal = noneVal.
+  Proof. unfold noneVal; simpl; rewrite tautology_6; trivial. Qed.
+
+End NoneAlwaysFalse.
 
 Module InfLeqRelation (VAL : SEM_VAL) (S: NONE_RELATION VAL) <: LEQ_RELATION ZInfinity VAL.
   Import ZInfinity.
@@ -231,8 +385,8 @@ Module InfLeqRelation (VAL : SEM_VAL) (S: NONE_RELATION VAL) <: LEQ_RELATION ZIn
   (* Definition of relation "less than or equal to" *)
   Definition num_leq (ze1 ze2 : A) : Val :=
     match ze1, ze2 with
-      | None, x                            => none_leq x
-      | x, None                            => leq_none x
+      | None, _
+      | _, None                            => noneVal
       | _, Some ZE_Inf                     => bool_inj true
       | Some ZE_NegInf, _                  => bool_inj true
       | Some ZE_Inf, Some x                => if ZE_eq_dec x ZE_Inf then bool_inj true else bool_inj false
@@ -262,8 +416,8 @@ Module PureInfinity <: SEMANTICS_INPUT.
   Definition QT (q : Q) : Type := match q with Q_Z => Z | Q_ZE => ZE end.
   Definition conv {q : Q} (x : QT q) : A :=
     match q return (QT q -> A) with
-     | Q_Z => fun x : Z => Some (ZE_Fin x)
-     | Q_ZE => fun x : ZE => Some x
+      | Q_Z => fun x : Z => Some (ZE_Fin x)
+      | Q_ZE => fun x : ZE => Some x
     end x.
 End PureInfinity.
 
@@ -285,466 +439,466 @@ Module IntToInfinity <: SEMANTICS_INPUT.
 End IntToInfinity.
 
 Module ArithSemantics (I : SEMANTICS_INPUT) (V : VARIABLE) (VAL : SEM_VAL) (S: NONE_RELATION VAL) (L : LEQ_RELATION I.N VAL).
-Import I N V VAL S L.
+  Import I N V VAL S L.
 
-(* Syntax *)
-Section OriginalForm.
+  (* Syntax *)
+  Section OriginalForm.
 
-  (* Arithmetic Expression *)
-  Inductive ZExp : Type :=
-  | ZExp_Var     : var  -> ZExp
-  | ZExp_Const   : A    -> ZExp
-  | ZExp_Add     : ZExp -> ZExp -> ZExp (* + *)
-  | ZExp_Inv     : ZExp -> ZExp (* unary - *)
-  | ZExp_Sub     : ZExp -> ZExp -> ZExp (* - *)
-  | ZExp_Mult    : Z    -> ZExp -> ZExp. (* Constant Multiplication *)
+    (* Arithmetic Expression *)
+    Inductive ZExp : Type :=
+    | ZExp_Var     : var  -> ZExp
+    | ZExp_Const   : A    -> ZExp
+    | ZExp_Add     : ZExp -> ZExp -> ZExp (* + *)
+    | ZExp_Inv     : ZExp -> ZExp (* unary - *)
+    | ZExp_Sub     : ZExp -> ZExp -> ZExp (* - *)
+    | ZExp_Mult    : Z    -> ZExp -> ZExp. (* Constant Multiplication *)
 
-  (* Boolean Forms *)
-  Inductive ZBF : Type :=
-  | ZBF_Const   : Val -> ZBF
-  | ZBF_Lt      : ZExp -> ZExp -> ZBF (* < *)
-  | ZBF_Lte     : ZExp -> ZExp -> ZBF (* <= *)
-  | ZBF_Gt      : ZExp -> ZExp -> ZBF (* > *)
-  | ZBF_Gte     : ZExp -> ZExp -> ZBF (* >= *)
-  | ZBF_Eq      : ZExp -> ZExp -> ZBF (* = *)
-  | ZBF_Eq_Max  : ZExp -> ZExp -> ZExp -> ZBF (* a = min(b, c) *)
-  | ZBF_Eq_Min  : ZExp -> ZExp -> ZExp -> ZBF (* a = max(b, c) *)
-  | ZBF_Neq     : ZExp -> ZExp -> ZBF. (* <> *)
+    (* Boolean Forms *)
+    Inductive ZBF : Type :=
+    | ZBF_Const   : Val -> ZBF
+    | ZBF_Lt      : ZExp -> ZExp -> ZBF (* < *)
+    | ZBF_Lte     : ZExp -> ZExp -> ZBF (* <= *)
+    | ZBF_Gt      : ZExp -> ZExp -> ZBF (* > *)
+    | ZBF_Gte     : ZExp -> ZExp -> ZBF (* >= *)
+    | ZBF_Eq      : ZExp -> ZExp -> ZBF (* = *)
+    | ZBF_Eq_Max  : ZExp -> ZExp -> ZExp -> ZBF (* a = min(b, c) *)
+    | ZBF_Eq_Min  : ZExp -> ZExp -> ZExp -> ZBF (* a = max(b, c) *)
+    | ZBF_Neq     : ZExp -> ZExp -> ZBF. (* <> *)
 
-  (* Logic Forms *)
-  Inductive ZF : Type :=
-  | ZF_BF      : ZBF -> ZF
-  | ZF_And     : ZF  -> ZF -> ZF (* /\ *)
-  | ZF_Or      : ZF  -> ZF -> ZF (* \/ *)
-  | ZF_Imp     : ZF  -> ZF -> ZF (* -> *)
-  | ZF_Not     : ZF  -> ZF       (* ~ *)
-  | ZF_Forall  : var -> Q -> ZF -> ZF  (* forall *)
-  | ZF_Exists  : var -> Q -> ZF -> ZF. (* exists *)
+    (* Logic Forms *)
+    Inductive ZF : Type :=
+    | ZF_BF      : ZBF -> ZF
+    | ZF_And     : ZF  -> ZF -> ZF (* /\ *)
+    | ZF_Or      : ZF  -> ZF -> ZF (* \/ *)
+    | ZF_Imp     : ZF  -> ZF -> ZF (* -> *)
+    | ZF_Not     : ZF  -> ZF       (* ~ *)
+    | ZF_Forall  : var -> Q -> ZF -> ZF  (* forall *)
+    | ZF_Exists  : var -> Q -> ZF -> ZF. (* exists *)
 
-End OriginalForm.
+  End OriginalForm.
 
-(* Semantics *)
-Section DirectSemantics.
+  (* Semantics *)
+  Section DirectSemantics.
 
-  (* Definition of constant multiplication of natural numbers *)
-  Fixpoint num_mult_nat (n : nat) (x : A) : A :=
-    match n with
-      | O   => Const0
-      | S n => num_plus x (num_mult_nat n x)
-    end.
+    (* Definition of constant multiplication of natural numbers *)
+    Fixpoint num_mult_nat (n : nat) (x : A) : A :=
+      match n with
+        | O   => Const0
+        | S n => num_plus x (num_mult_nat n x)
+      end.
 
-  (* Definition of constant multiplication of integers *)
-  Definition num_mult (z : Z) (exp : A) : A :=
-    match z with
-      | Z0     => Const0
-      | Zpos x => num_mult_nat (nat_of_P x) exp
-      | Zneg x => num_neg (num_mult_nat (nat_of_P x) exp)
-    end.
+    (* Definition of constant multiplication of integers *)
+    Definition num_mult (z : Z) (exp : A) : A :=
+      match z with
+        | Z0     => Const0
+        | Zpos x => num_mult_nat (nat_of_P x) exp
+        | Zneg x => num_neg (num_mult_nat (nat_of_P x) exp)
+      end.
 
-  (* Substitution on Expressions *)
-  Fixpoint subst_exp (p : var * A) (exp : ZExp) : ZExp :=
-    match exp with
-        ZExp_Var v     => if var_eq_dec (fst p) v then ZExp_Const (snd p) else exp
-      | ZExp_Const _   => exp
-      | ZExp_Add e1 e2 => ZExp_Add (subst_exp p e1) (subst_exp p e2)
-      | ZExp_Inv e     => ZExp_Inv (subst_exp p e)
-      | ZExp_Sub e1 e2 => ZExp_Sub (subst_exp p e1) (subst_exp p e2)
-      | ZExp_Mult n e  => ZExp_Mult n (subst_exp p e)
-    end.
+    (* Substitution on Expressions *)
+    Fixpoint subst_exp (p : var * A) (exp : ZExp) : ZExp :=
+      match exp with
+          ZExp_Var v     => if var_eq_dec (fst p) v then ZExp_Const (snd p) else exp
+        | ZExp_Const _   => exp
+        | ZExp_Add e1 e2 => ZExp_Add (subst_exp p e1) (subst_exp p e2)
+        | ZExp_Inv e     => ZExp_Inv (subst_exp p e)
+        | ZExp_Sub e1 e2 => ZExp_Sub (subst_exp p e1) (subst_exp p e2)
+        | ZExp_Mult n e  => ZExp_Mult n (subst_exp p e)
+      end.
 
-  (* Substitution on Boolean Forms *)
-  Fixpoint subst_bf (p : var * A) (bf : ZBF) : ZBF :=
-    match bf with
-        ZBF_Const _   => bf
-      | ZBF_Lt e1 e2  => ZBF_Lt (subst_exp p e1) (subst_exp p e2)
-      | ZBF_Lte e1 e2 => ZBF_Lte (subst_exp p e1) (subst_exp p e2)
-      | ZBF_Gt e1 e2  => ZBF_Gt (subst_exp p e1) (subst_exp p e2)
-      | ZBF_Gte e1 e2 => ZBF_Gte (subst_exp p e1) (subst_exp p e2)
-      | ZBF_Eq e1 e2  => ZBF_Eq (subst_exp p e1) (subst_exp p e2)
-      | ZBF_Eq_Max e1 e2 e3  => ZBF_Eq_Max (subst_exp p e1) (subst_exp p e2) (subst_exp p e3)
-      | ZBF_Eq_Min e1 e2 e3  => ZBF_Eq_Min (subst_exp p e1) (subst_exp p e2) (subst_exp p e3)
-      | ZBF_Neq e1 e2 => ZBF_Neq (subst_exp p e1) (subst_exp p e2)
-    end.
+    (* Substitution on Boolean Forms *)
+    Fixpoint subst_bf (p : var * A) (bf : ZBF) : ZBF :=
+      match bf with
+          ZBF_Const _   => bf
+        | ZBF_Lt e1 e2  => ZBF_Lt (subst_exp p e1) (subst_exp p e2)
+        | ZBF_Lte e1 e2 => ZBF_Lte (subst_exp p e1) (subst_exp p e2)
+        | ZBF_Gt e1 e2  => ZBF_Gt (subst_exp p e1) (subst_exp p e2)
+        | ZBF_Gte e1 e2 => ZBF_Gte (subst_exp p e1) (subst_exp p e2)
+        | ZBF_Eq e1 e2  => ZBF_Eq (subst_exp p e1) (subst_exp p e2)
+        | ZBF_Eq_Max e1 e2 e3  => ZBF_Eq_Max (subst_exp p e1) (subst_exp p e2) (subst_exp p e3)
+        | ZBF_Eq_Min e1 e2 e3  => ZBF_Eq_Min (subst_exp p e1) (subst_exp p e2) (subst_exp p e3)
+        | ZBF_Neq e1 e2 => ZBF_Neq (subst_exp p e1) (subst_exp p e2)
+      end.
 
-  (* Substitution on Logic Forms *)
-  Fixpoint substitute (p : var * A) (form : ZF) : ZF :=
-    match form with
-        ZF_BF bf      => ZF_BF (subst_bf p bf)
-      | ZF_And f1 f2  => ZF_And (substitute p f1) (substitute p f2)
-      | ZF_Or f1 f2   => ZF_Or (substitute p f1) (substitute p f2)
-      | ZF_Imp f1 f2  => ZF_Imp (substitute p f1) (substitute p f2)
-      | ZF_Not f      => ZF_Not (substitute p f)
-      | ZF_Forall v q f => if var_eq_dec (fst p) v then form else ZF_Forall v q (substitute p f)
-      | ZF_Exists v q f => if var_eq_dec (fst p) v then form else ZF_Exists v q (substitute p f)
-    end.
+    (* Substitution on Logic Forms *)
+    Fixpoint substitute (p : var * A) (form : ZF) : ZF :=
+      match form with
+          ZF_BF bf      => ZF_BF (subst_bf p bf)
+        | ZF_And f1 f2  => ZF_And (substitute p f1) (substitute p f2)
+        | ZF_Or f1 f2   => ZF_Or (substitute p f1) (substitute p f2)
+        | ZF_Imp f1 f2  => ZF_Imp (substitute p f1) (substitute p f2)
+        | ZF_Not f      => ZF_Not (substitute p f)
+        | ZF_Forall v q f => if var_eq_dec (fst p) v then form else ZF_Forall v q (substitute p f)
+        | ZF_Exists v q f => if var_eq_dec (fst p) v then form else ZF_Exists v q (substitute p f)
+      end.
 
-  (* For the same variable, second substitution on expressions has no effect. *)
-  Lemma same_var_subst_exp: forall exp v a1 a2, subst_exp (v, a1) (subst_exp (v, a2) exp) = subst_exp (v, a2) exp.
-  Proof.
-    induction exp; simpl; intros.
-    destruct (var_eq_dec v0 v); simpl; auto.
-    destruct (var_eq_dec v0 v); simpl; tauto.
-    auto.
-    rewrite IHexp1, IHexp2; auto.
-    rewrite IHexp; auto.
-    rewrite IHexp1, IHexp2; auto.
-    rewrite IHexp; auto.
-  Qed.
+    (* For the same variable, second substitution on expressions has no effect. *)
+    Lemma same_var_subst_exp: forall exp v a1 a2, subst_exp (v, a1) (subst_exp (v, a2) exp) = subst_exp (v, a2) exp.
+    Proof.
+      induction exp; simpl; intros.
+      destruct (var_eq_dec v0 v); simpl; auto.
+      destruct (var_eq_dec v0 v); simpl; tauto.
+      auto.
+      rewrite IHexp1, IHexp2; auto.
+      rewrite IHexp; auto.
+      rewrite IHexp1, IHexp2; auto.
+      rewrite IHexp; auto.
+    Qed.
 
-  (* For the same variable, second substitution on boolean forms has no effect. *)
-  Lemma same_var_subst_bf: forall bf v a1 a2, subst_bf (v, a1) (subst_bf (v, a2) bf) = subst_bf (v, a2) bf.
-  Proof.
-    destruct bf; simpl; intros; auto;
-    try (rewrite same_var_subst_exp, same_var_subst_exp, same_var_subst_exp; auto);
-    try (rewrite same_var_subst_exp, same_var_subst_exp; auto).
-  Qed.
+    (* For the same variable, second substitution on boolean forms has no effect. *)
+    Lemma same_var_subst_bf: forall bf v a1 a2, subst_bf (v, a1) (subst_bf (v, a2) bf) = subst_bf (v, a2) bf.
+    Proof.
+      destruct bf; simpl; intros; auto;
+      try (rewrite same_var_subst_exp, same_var_subst_exp, same_var_subst_exp; auto);
+      try (rewrite same_var_subst_exp, same_var_subst_exp; auto).
+    Qed.
 
-  (* For the same variable, second substitution on logic forms has no effect. *)
-  Lemma same_var_subst: forall f v a1 a2, substitute (v, a1) (substitute (v, a2) f) = substitute (v, a2) f.
-  Proof.
-    induction f; intros;
-    try (unfold substitute; rewrite same_var_subst_bf; auto);
-    try (unfold substitute; fold substitute; rewrite IHf1, IHf2; auto);
-    try (unfold substitute; fold substitute; rewrite IHf; auto);
-    try (unfold substitute; fold substitute; unfold fst;
-    destruct (var_eq_dec v0 v);
-    unfold substitute; fold substitute; unfold fst;
-    destruct (var_eq_dec v0 v); auto; try tauto;
-    rewrite IHf; auto).
-  Qed.
+    (* For the same variable, second substitution on logic forms has no effect. *)
+    Lemma same_var_subst: forall f v a1 a2, substitute (v, a1) (substitute (v, a2) f) = substitute (v, a2) f.
+    Proof.
+      induction f; intros;
+      try (unfold substitute; rewrite same_var_subst_bf; auto);
+      try (unfold substitute; fold substitute; rewrite IHf1, IHf2; auto);
+      try (unfold substitute; fold substitute; rewrite IHf; auto);
+      try (unfold substitute; fold substitute; unfold fst;
+           destruct (var_eq_dec v0 v);
+           unfold substitute; fold substitute; unfold fst;
+           destruct (var_eq_dec v0 v); auto; try tauto;
+           rewrite IHf; auto).
+    Qed.
 
-  (* Commutative law for substitution on expressions with different variables *)
-  Lemma diff_var_subst_exp: forall exp v1 v2 a1 a2, v1 <> v2 -> subst_exp (v1, a1) (subst_exp (v2, a2) exp) =
-                                                                subst_exp (v2, a2) (subst_exp (v1, a1) exp).
-  Proof.
-    induction exp; simpl; intros.
-    destruct (var_eq_dec v2 v), (var_eq_dec v1 v).
-    rewrite <- e in e0; tauto.
-    simpl; destruct (var_eq_dec v2 v); tauto.
-    simpl; destruct (var_eq_dec v1 v); tauto.
-    simpl. destruct (var_eq_dec v2 v), (var_eq_dec v1 v); tauto.
-    auto.
-    rewrite IHexp1, IHexp2; auto.
-    rewrite IHexp; auto.
-    rewrite IHexp1, IHexp2; auto.
-    rewrite IHexp; auto.
-  Qed.
+    (* Commutative law for substitution on expressions with different variables *)
+    Lemma diff_var_subst_exp: forall exp v1 v2 a1 a2, v1 <> v2 -> subst_exp (v1, a1) (subst_exp (v2, a2) exp) =
+                                                                  subst_exp (v2, a2) (subst_exp (v1, a1) exp).
+    Proof.
+      induction exp; simpl; intros.
+      destruct (var_eq_dec v2 v), (var_eq_dec v1 v).
+      rewrite <- e in e0; tauto.
+      simpl; destruct (var_eq_dec v2 v); tauto.
+      simpl; destruct (var_eq_dec v1 v); tauto.
+      simpl. destruct (var_eq_dec v2 v), (var_eq_dec v1 v); tauto.
+      auto.
+      rewrite IHexp1, IHexp2; auto.
+      rewrite IHexp; auto.
+      rewrite IHexp1, IHexp2; auto.
+      rewrite IHexp; auto.
+    Qed.
 
-  (* Commutative law for substitution on boolean forms with different variables *)
-  Lemma diff_var_subst_bf: forall bf v1 v2 a1 a2, v1 <> v2 -> subst_bf (v1, a1) (subst_bf (v2, a2) bf) =
-                                                              subst_bf (v2, a2) (subst_bf (v1, a1) bf).
-  Proof.
-    destruct bf; simpl; intros; auto;
-    (rewrite diff_var_subst_exp  with (exp := z);
-     try rewrite diff_var_subst_exp with (exp := z0);
-     try rewrite diff_var_subst_exp with (exp := z1);
-     auto).
-  Qed.
+    (* Commutative law for substitution on boolean forms with different variables *)
+    Lemma diff_var_subst_bf: forall bf v1 v2 a1 a2, v1 <> v2 -> subst_bf (v1, a1) (subst_bf (v2, a2) bf) =
+                                                                subst_bf (v2, a2) (subst_bf (v1, a1) bf).
+    Proof.
+      destruct bf; simpl; intros; auto;
+      (rewrite diff_var_subst_exp  with (exp := z);
+       try rewrite diff_var_subst_exp with (exp := z0);
+       try rewrite diff_var_subst_exp with (exp := z1);
+       auto).
+    Qed.
 
-  (* Commutative law for substitution on logic forms with different variables *)
-  Lemma diff_var_subst: forall f v1 v2 a1 a2, v1 <> v2 -> substitute (v1, a1) (substitute (v2, a2) f) =
-                                                          substitute (v2, a2) (substitute (v1, a1) f).
-  Proof.
-    induction f; intros;
-    try (unfold substitute; rewrite diff_var_subst_bf; auto);
-    try (unfold substitute; fold substitute; rewrite IHf1, IHf2; auto);
-    try (unfold substitute; fold substitute; rewrite IHf; auto);
-    (unfold substitute; fold substitute; unfold fst;
-     destruct (var_eq_dec v2 v), (var_eq_dec v1 v); auto;
-     try (rewrite <- e in e0; tauto);
-     try (simpl; destruct (var_eq_dec v2 v), (var_eq_dec v1 v); try tauto);
-     rewrite IHf; auto).
-  Qed.
+    (* Commutative law for substitution on logic forms with different variables *)
+    Lemma diff_var_subst: forall f v1 v2 a1 a2, v1 <> v2 -> substitute (v1, a1) (substitute (v2, a2) f) =
+                                                            substitute (v2, a2) (substitute (v1, a1) f).
+    Proof.
+      induction f; intros;
+      try (unfold substitute; rewrite diff_var_subst_bf; auto);
+      try (unfold substitute; fold substitute; rewrite IHf1, IHf2; auto);
+      try (unfold substitute; fold substitute; rewrite IHf; auto);
+      (unfold substitute; fold substitute; unfold fst;
+       destruct (var_eq_dec v2 v), (var_eq_dec v1 v); auto;
+       try (rewrite <- e in e0; tauto);
+       try (simpl; destruct (var_eq_dec v2 v), (var_eq_dec v1 v); try tauto);
+       rewrite IHf; auto).
+    Qed.
 
-  (* Evaluation of Expressions *)
-  Fixpoint dexp2ZE (exp : ZExp) : A :=
-    match exp with
-        ZExp_Var _     => Const0
-      | ZExp_Const z   => z
-      | ZExp_Add e1 e2 => num_plus (dexp2ZE e1) (dexp2ZE e2)
-      | ZExp_Inv e     => num_neg (dexp2ZE e)
-      | ZExp_Sub e1 e2 => num_plus (dexp2ZE e1) (num_neg (dexp2ZE e2))
-      | ZExp_Mult z e  => num_mult z (dexp2ZE e)
-    end.
+    (* Evaluation of Expressions *)
+    Fixpoint dexp2ZE (exp : ZExp) : A :=
+      match exp with
+          ZExp_Var _     => Const0
+        | ZExp_Const z   => z
+        | ZExp_Add e1 e2 => num_plus (dexp2ZE e1) (dexp2ZE e2)
+        | ZExp_Inv e     => num_neg (dexp2ZE e)
+        | ZExp_Sub e1 e2 => num_plus (dexp2ZE e1) (num_neg (dexp2ZE e2))
+        | ZExp_Mult z e  => num_mult z (dexp2ZE e)
+      end.
 
-  (* Evaluation of Boolean Forms *)
-  Fixpoint dzbf2bool (bf : ZBF) : Val :=
-    match bf with
-        ZBF_Const b   => b
-      | ZBF_Lt e1 e2  => let v1 := dexp2ZE e1 in
-                         let v2 := dexp2ZE e2 in
-                         truth_and (num_leq v1 v2) (truth_not (num_leq v2 v1))
-      | ZBF_Lte e1 e2 => num_leq (dexp2ZE e1) (dexp2ZE e2)
-      | ZBF_Gt e1 e2  => let v1 := dexp2ZE e1 in
-                         let v2 := dexp2ZE e2 in
-                         truth_and (num_leq v2 v1) (truth_not (num_leq v1 v2))
-      | ZBF_Gte e1 e2 => num_leq (dexp2ZE e2) (dexp2ZE e1)
-      | ZBF_Eq e1 e2  => let v1 := dexp2ZE e1 in
-                         let v2 := dexp2ZE e2 in
-                         truth_and (num_leq v1 v2) (num_leq v2 v1)
-      | ZBF_Eq_Max e1 e2 e3 =>
-                         let v1 := dexp2ZE e1 in
-                         let v2 := dexp2ZE e2 in
-                         let v3 := dexp2ZE e3 in
-                         truth_or (truth_and (num_leq v3 v2) (truth_and (num_leq v1 v2) (num_leq v2 v1)))
-                                  (truth_and (num_leq v2 v3) (truth_and (num_leq v1 v3) (num_leq v3 v1)))
-      | ZBF_Eq_Min e1 e2 e3 =>
-                         let v1 := dexp2ZE e1 in
-                         let v2 := dexp2ZE e2 in
-                         let v3 := dexp2ZE e3 in
-                         truth_or (truth_and (num_leq v3 v2) (truth_and (num_leq v1 v3) (num_leq v3 v1)))
-                                  (truth_and (num_leq v2 v3) (truth_and (num_leq v1 v2) (num_leq v2 v1)))
-      | ZBF_Neq e1 e2 => let v1 := dexp2ZE e1 in
-                         let v2 := dexp2ZE e2 in
-                         truth_not (truth_and (num_leq v1 v2) (num_leq v2 v1))
-    end.
+    (* Evaluation of Boolean Forms *)
+    Fixpoint dzbf2bool (bf : ZBF) : Val :=
+      match bf with
+          ZBF_Const b   => b
+        | ZBF_Lt e1 e2  => let v1 := dexp2ZE e1 in
+                           let v2 := dexp2ZE e2 in
+                           truth_and (num_leq v1 v2) (truth_not (num_leq v2 v1))
+        | ZBF_Lte e1 e2 => num_leq (dexp2ZE e1) (dexp2ZE e2)
+        | ZBF_Gt e1 e2  => let v1 := dexp2ZE e1 in
+                           let v2 := dexp2ZE e2 in
+                           truth_and (num_leq v2 v1) (truth_not (num_leq v1 v2))
+        | ZBF_Gte e1 e2 => num_leq (dexp2ZE e2) (dexp2ZE e1)
+        | ZBF_Eq e1 e2  => let v1 := dexp2ZE e1 in
+                           let v2 := dexp2ZE e2 in
+                           truth_and (num_leq v1 v2) (num_leq v2 v1)
+        | ZBF_Eq_Max e1 e2 e3 =>
+          let v1 := dexp2ZE e1 in
+          let v2 := dexp2ZE e2 in
+          let v3 := dexp2ZE e3 in
+          truth_or (truth_and (num_leq v3 v2) (truth_and (num_leq v1 v2) (num_leq v2 v1)))
+                   (truth_and (num_leq v2 v3) (truth_and (num_leq v1 v3) (num_leq v3 v1)))
+        | ZBF_Eq_Min e1 e2 e3 =>
+          let v1 := dexp2ZE e1 in
+          let v2 := dexp2ZE e2 in
+          let v3 := dexp2ZE e3 in
+          truth_or (truth_and (num_leq v3 v2) (truth_and (num_leq v1 v3) (num_leq v3 v1)))
+                   (truth_and (num_leq v2 v3) (truth_and (num_leq v1 v2) (num_leq v2 v1)))
+        | ZBF_Neq e1 e2 => let v1 := dexp2ZE e1 in
+                           let v2 := dexp2ZE e2 in
+                           truth_not (truth_and (num_leq v1 v2) (num_leq v2 v1))
+      end.
 
-  (* Length of Logic Form *)
-  Fixpoint length_zform (form : ZF) : nat :=
-    match form with
-        ZF_BF _       => 1
-      | ZF_And f1 f2  => S (length_zform f1 + length_zform f2)
-      | ZF_Or f1 f2   => S (length_zform f1 + length_zform f2)
-      | ZF_Imp f1 f2  => S (length_zform f1 + length_zform f2)
-      | ZF_Not f      => S (length_zform f)
-      | ZF_Forall _ _ f => S (length_zform f)
-      | ZF_Exists _ _ f => S (length_zform f)
-    end.
+    (* Length of Logic Form *)
+    Fixpoint length_zform (form : ZF) : nat :=
+      match form with
+          ZF_BF _       => 1
+        | ZF_And f1 f2  => S (length_zform f1 + length_zform f2)
+        | ZF_Or f1 f2   => S (length_zform f1 + length_zform f2)
+        | ZF_Imp f1 f2  => S (length_zform f1 + length_zform f2)
+        | ZF_Not f      => S (length_zform f)
+        | ZF_Forall _ _ f => S (length_zform f)
+        | ZF_Exists _ _ f => S (length_zform f)
+      end.
 
-  (* Substitution doesn't change the length *)
-  Lemma substitute_length_inv : forall f x v, length_zform f = length_zform (substitute (v, x) f).
-  Proof.
-    induction f; simpl; try tauto; intros;
-    try (rewrite <- IHf1; rewrite <- IHf2);
-    try rewrite <- IHf;
-    try (case (var_eq_dec v0 v); intros; simpl); auto.
-  Defined.
+    (* Substitution doesn't change the length *)
+    Lemma substitute_length_inv : forall f x v, length_zform f = length_zform (substitute (v, x) f).
+    Proof.
+      induction f; simpl; try tauto; intros;
+      try (rewrite <- IHf1; rewrite <- IHf2);
+      try rewrite <- IHf;
+      try (case (var_eq_dec v0 v); intros; simpl); auto.
+    Defined.
 
-  (* Definition of Validity of Logic Forms *)
-  Inductive Input := Sat: ZF -> Input | DisSat: ZF -> Input | Undtmd: ZF -> Input.
+    (* Definition of Validity of Logic Forms *)
+    Inductive Input := Sat: ZF -> Input | DisSat: ZF -> Input | Udtmd: ZF -> Input.
 
-  Definition length_input (inp : Input) :=
-    match inp with
-      | Sat f => length_zform f
-      | DisSat f => length_zform f
-      | Undtmd f => length_zform f
-    end.
+    Definition length_input (inp : Input) :=
+      match inp with
+        | Sat f => length_zform f
+        | DisSat f => length_zform f
+        | Udtmd f => length_zform f
+      end.
 
-  Definition inputOrder (f1 f2 : Input) := length_input f1 < length_input f2.
+    Definition inputOrder (f1 f2 : Input) := length_input f1 < length_input f2.
 
-  Lemma inputOrder_wf': forall len f, length_input f <= len -> Acc inputOrder f.
-  Proof.
-    unfold inputOrder; induction len; intros;
-    [destruct f; destruct z; simpl in H; exfalso; intuition | constructor; intros; apply IHlen; omega].
-  Defined.
+    Lemma inputOrder_wf': forall len f, length_input f <= len -> Acc inputOrder f.
+    Proof.
+      unfold inputOrder; induction len; intros;
+      [destruct f; destruct z; simpl in H; exfalso; intuition | constructor; intros; apply IHlen; omega].
+    Defined.
 
-  Theorem inputOrder_wf: well_founded inputOrder.
-  Proof. red; intro; eapply inputOrder_wf'; eauto. Defined.
+    Theorem inputOrder_wf: well_founded inputOrder.
+    Proof. red; intro; eapply inputOrder_wf'; eauto. Defined.
 
-  Ltac smash := intros; unfold inputOrder; simpl; omega || rewrite <- substitute_length_inv; omega.
+    Ltac smash := intros; unfold inputOrder; simpl; omega || rewrite <- substitute_length_inv; omega.
 
-  Lemma sat_and_1: forall f1 f2, inputOrder (Sat f1) (Sat (ZF_And f1 f2)). smash. Defined.
-  Lemma sat_and_2: forall f1 f2, inputOrder (Sat f2) (Sat (ZF_And f1 f2)). smash. Defined.
-  Lemma sat_or_1: forall f1 f2, inputOrder (Sat f1) (Sat (ZF_Or f1 f2)). smash. Defined.
-  Lemma sat_or_2: forall f1 f2, inputOrder (Sat f2) (Sat (ZF_Or f1 f2)). smash. Defined.
-  Lemma sat_imp_1: forall f1 f2, inputOrder (DisSat f1) (Sat (ZF_Imp f1 f2)). smash. Defined.
-  Lemma sat_imp_2: forall f1 f2, inputOrder (Sat f2) (Sat (ZF_Imp f1 f2)). smash. Defined.
-  Lemma sat_not : forall f, inputOrder (DisSat f) (Sat (ZF_Not f)). smash. Defined.
-  Lemma sat_forall:forall f v q(x:QT q),inputOrder(Sat (substitute (v, @conv q x) f))(Sat (ZF_Forall v q f)). smash. Defined.
-  Lemma sat_exists:forall f v q(x:QT q),inputOrder(Sat (substitute (v, @conv q x) f))(Sat (ZF_Exists v q f)). smash. Defined.
-  Lemma dst_and_1: forall f1 f2, inputOrder (DisSat f1) (DisSat (ZF_And f1 f2)). smash. Defined.
-  Lemma dst_and_2: forall f1 f2, inputOrder (DisSat f2) (DisSat (ZF_And f1 f2)). smash. Defined.
-  Lemma dst_or_1: forall f1 f2, inputOrder (DisSat f1) (DisSat (ZF_Or f1 f2)). smash. Defined.
-  Lemma dst_or_2: forall f1 f2, inputOrder (DisSat f2) (DisSat (ZF_Or f1 f2)). smash. Defined.
-  Lemma dst_imp_1: forall f1 f2, inputOrder (Sat f1) (DisSat (ZF_Imp f1 f2)). smash. Defined.
-  Lemma dst_imp_2: forall f1 f2, inputOrder (DisSat f2) (DisSat (ZF_Imp f1 f2)). smash. Defined.
-  Lemma dst_not : forall f, inputOrder (Sat f) (DisSat (ZF_Not f)). smash. Defined.
-  Lemma dst_forall:forall f v q(x:QT q),inputOrder(DisSat(substitute (v,@conv q x) f))(Sat (ZF_Forall v q f)). smash. Defined.
-  Lemma dst_exists:forall f v q(x:QT q),inputOrder(DisSat(substitute (v,@conv q x) f))(Sat (ZF_Exists v q f)). smash. Defined.
-  Lemma udd_and_1 : forall f1 f2, inputOrder (Sat f1) (Undtmd (ZF_And f1 f2)). smash. Defined.
-  Lemma udd_and_2 : forall f1 f2, inputOrder (Sat f2) (Undtmd (ZF_And f1 f2)). smash. Defined.
-  Lemma udd_and_3 : forall f1 f2, inputOrder (DisSat f1) (Undtmd (ZF_And f1 f2)). smash. Defined.
-  Lemma udd_and_4 : forall f1 f2, inputOrder (DisSat f2) (Undtmd (ZF_And f1 f2)). smash. Defined.
-  Lemma udd_or_1 : forall f1 f2, inputOrder (Sat f1) (Undtmd (ZF_Or f1 f2)). smash. Defined.
-  Lemma udd_or_2 : forall f1 f2, inputOrder (Sat f2) (Undtmd (ZF_Or f1 f2)). smash. Defined.
-  Lemma udd_or_3 : forall f1 f2, inputOrder (DisSat f1) (Undtmd (ZF_Or f1 f2)). smash. Defined.
-  Lemma udd_or_4 : forall f1 f2, inputOrder (DisSat f2) (Undtmd (ZF_Or f1 f2)). smash. Defined.
-  Lemma udd_imp_1 : forall f1 f2, inputOrder (DisSat f1) (Undtmd (ZF_Imp f1 f2)). smash. Defined.
-  Lemma udd_imp_2 : forall f1 f2, inputOrder (Sat f2) (Undtmd (ZF_Imp f1 f2)). smash. Defined.
-  Lemma udd_imp_3 : forall f1 f2, inputOrder (Sat f1) (Undtmd (ZF_Imp f1 f2)). smash. Defined.
-  Lemma udd_imp_4 : forall f1 f2, inputOrder (DisSat f2) (Undtmd (ZF_Imp f1 f2)). smash. Defined.
-  Lemma udd_not_1 : forall f, inputOrder (DisSat f) (Undtmd (ZF_Not f)). smash. Defined.
-  Lemma udd_not_2 : forall f, inputOrder (Sat f) (Undtmd (ZF_Not f)). smash. Defined.
-  Lemma udd_forall_1:forall f v q(x:QT q),inputOrder(Sat(substitute(v,@conv q x)f))(Undtmd(ZF_Forall v q f)). smash. Defined.
-  Lemma udd_forall_2:forall f v q(x:QT q),inputOrder(DisSat(substitute(v,@conv q x)f))(Undtmd(ZF_Forall v q f)). smash. Defined.
-  Lemma udd_exists_1:forall f v q(x:QT q),inputOrder(Sat(substitute(v,@conv q x)f))(Undtmd(ZF_Exists v q f)). smash. Defined.
-  Lemma udd_exists_2:forall f v q(x:QT q),inputOrder(DisSat(substitute(v,@conv q x)f))(Undtmd(ZF_Exists v q f)). smash. Defined.
+    Lemma sat_and_1: forall f1 f2, inputOrder (Sat f1) (Sat (ZF_And f1 f2)). smash. Defined.
+    Lemma sat_and_2: forall f1 f2, inputOrder (Sat f2) (Sat (ZF_And f1 f2)). smash. Defined.
+    Lemma sat_or_1: forall f1 f2, inputOrder (Sat f1) (Sat (ZF_Or f1 f2)). smash. Defined.
+    Lemma sat_or_2: forall f1 f2, inputOrder (Sat f2) (Sat (ZF_Or f1 f2)). smash. Defined.
+    Lemma sat_imp_1: forall f1 f2, inputOrder (DisSat f1) (Sat (ZF_Imp f1 f2)). smash. Defined.
+    Lemma sat_imp_2: forall f1 f2, inputOrder (Sat f2) (Sat (ZF_Imp f1 f2)). smash. Defined.
+    Lemma sat_not : forall f, inputOrder (DisSat f) (Sat (ZF_Not f)). smash. Defined.
+    Lemma sat_forall:forall f v q(x:QT q),inputOrder(Sat (substitute (v, @conv q x) f))(Sat (ZF_Forall v q f)). smash. Defined.
+    Lemma sat_exists:forall f v q(x:QT q),inputOrder(Sat (substitute (v, @conv q x) f))(Sat (ZF_Exists v q f)). smash. Defined.
+    Lemma dst_and_1: forall f1 f2, inputOrder (DisSat f1) (DisSat (ZF_And f1 f2)). smash. Defined.
+    Lemma dst_and_2: forall f1 f2, inputOrder (DisSat f2) (DisSat (ZF_And f1 f2)). smash. Defined.
+    Lemma dst_or_1: forall f1 f2, inputOrder (DisSat f1) (DisSat (ZF_Or f1 f2)). smash. Defined.
+    Lemma dst_or_2: forall f1 f2, inputOrder (DisSat f2) (DisSat (ZF_Or f1 f2)). smash. Defined.
+    Lemma dst_imp_1: forall f1 f2, inputOrder (Sat f1) (DisSat (ZF_Imp f1 f2)). smash. Defined.
+    Lemma dst_imp_2: forall f1 f2, inputOrder (DisSat f2) (DisSat (ZF_Imp f1 f2)). smash. Defined.
+    Lemma dst_not : forall f, inputOrder (Sat f) (DisSat (ZF_Not f)). smash. Defined.
+    Lemma dst_forall:forall f v q(x:QT q),inputOrder(DisSat(substitute (v,@conv q x) f))(Sat (ZF_Forall v q f)). smash. Defined.
+    Lemma dst_exists:forall f v q(x:QT q),inputOrder(DisSat(substitute (v,@conv q x) f))(Sat (ZF_Exists v q f)). smash. Defined.
+    Lemma udd_and_1 : forall f1 f2, inputOrder (Sat f1) (Udtmd (ZF_And f1 f2)). smash. Defined.
+    Lemma udd_and_2 : forall f1 f2, inputOrder (Sat f2) (Udtmd (ZF_And f1 f2)). smash. Defined.
+    Lemma udd_and_3 : forall f1 f2, inputOrder (DisSat f1) (Udtmd (ZF_And f1 f2)). smash. Defined.
+    Lemma udd_and_4 : forall f1 f2, inputOrder (DisSat f2) (Udtmd (ZF_And f1 f2)). smash. Defined.
+    Lemma udd_or_1 : forall f1 f2, inputOrder (Sat f1) (Udtmd (ZF_Or f1 f2)). smash. Defined.
+    Lemma udd_or_2 : forall f1 f2, inputOrder (Sat f2) (Udtmd (ZF_Or f1 f2)). smash. Defined.
+    Lemma udd_or_3 : forall f1 f2, inputOrder (DisSat f1) (Udtmd (ZF_Or f1 f2)). smash. Defined.
+    Lemma udd_or_4 : forall f1 f2, inputOrder (DisSat f2) (Udtmd (ZF_Or f1 f2)). smash. Defined.
+    Lemma udd_imp_1 : forall f1 f2, inputOrder (DisSat f1) (Udtmd (ZF_Imp f1 f2)). smash. Defined.
+    Lemma udd_imp_2 : forall f1 f2, inputOrder (Sat f2) (Udtmd (ZF_Imp f1 f2)). smash. Defined.
+    Lemma udd_imp_3 : forall f1 f2, inputOrder (Sat f1) (Udtmd (ZF_Imp f1 f2)). smash. Defined.
+    Lemma udd_imp_4 : forall f1 f2, inputOrder (DisSat f2) (Udtmd (ZF_Imp f1 f2)). smash. Defined.
+    Lemma udd_not_1 : forall f, inputOrder (DisSat f) (Udtmd (ZF_Not f)). smash. Defined.
+    Lemma udd_not_2 : forall f, inputOrder (Sat f) (Udtmd (ZF_Not f)). smash. Defined.
+    Lemma udd_forall_1:forall f v q(x:QT q),inputOrder(Sat(substitute(v,@conv q x)f))(Udtmd(ZF_Forall v q f)). smash. Defined.
+    Lemma udd_forall_2:forall f v q(x:QT q),inputOrder(DisSat(substitute(v,@conv q x)f))(Udtmd(ZF_Forall v q f)). smash. Defined.
+    Lemma udd_exists_1:forall f v q(x:QT q),inputOrder(Sat(substitute(v,@conv q x)f))(Udtmd(ZF_Exists v q f)). smash. Defined.
+    Lemma udd_exists_2:forall f v q(x:QT q),inputOrder(DisSat(substitute(v,@conv q x)f))(Udtmd(ZF_Exists v q f)). smash. Defined.
 
-  Definition three_pred : Input -> Prop :=
-    Fix inputOrder_wf (fun _ => Prop)
-        (fun (inp : Input) =>
-           match inp return ((forall ff : Input, inputOrder ff inp -> Prop) -> Prop) with
-             | Sat g =>
-               match g with
-                 | ZF_BF bf      => fun _ => dzbf2bool bf = bool_inj true
-                 | ZF_And f1 f2  => fun tpF => (tpF (Sat f1) (sat_and_1 f1 f2)) /\ (tpF (Sat f2) (sat_and_2 f1 f2))
-                 | ZF_Or f1 f2   => fun tpF => (tpF (Sat f1) (sat_or_1 f1 f2)) \/ (tpF (Sat f2) (sat_or_2 f1 f2))
-                 | ZF_Imp f1 f2  => fun tpF => (tpF (DisSat f1) (sat_imp_1 f1 f2)) \/ (tpF (Sat f2) (sat_imp_2 f1 f2))
-                 | ZF_Not f      => fun tpF => (tpF (DisSat f) (sat_not f))
-                 | ZF_Forall v q f => fun tpF => forall x : QT q, (tpF (Sat (substitute (v, @conv q x) f)) (sat_forall f v q x))
-                 | ZF_Exists v q f => fun tpF => exists x : QT q, (tpF (Sat (substitute (v, @conv q x) f)) (sat_exists f v q x))
-               end
-             | DisSat g =>
-               match g with
-                 | ZF_BF bf => fun _ => dzbf2bool bf = bool_inj false
-                 | ZF_And f1 f2 => fun tpF => (tpF (DisSat f1) (dst_and_1 f1 f2)) \/ (tpF (DisSat f2) (dst_and_2 f1 f2))
-                 | ZF_Or f1 f2 => fun tpF => (tpF (DisSat f1) (dst_or_1 f1 f2)) /\ (tpF (DisSat f2) (dst_or_2 f1 f2))
-                 | ZF_Imp f1 f2 => fun tpF => (tpF (Sat f1) (dst_imp_1 f1 f2)) /\ (tpF (DisSat f2) (dst_imp_2 f1 f2))
-                 | ZF_Not f => fun tpF => (tpF (Sat f) (dst_not f))
-                 | ZF_Forall v q f => fun tpF => exists x : QT q,
-                                                   (tpF (DisSat (substitute (v, @conv q x) f)) (dst_forall f v q x))
-                 | ZF_Exists v q f => fun tpF => forall x : QT q,
-                                                   (tpF (DisSat (substitute (v, @conv q x) f)) (dst_exists f v q x))
-               end
-             | Undtmd g =>
-               match g with
-                 | ZF_BF bf => fun _ => (dzbf2bool bf <> bool_inj true) /\ (dzbf2bool bf <> bool_inj false)
-                 | ZF_And f1 f2 => fun tpF => (~ ((tpF (Sat f1) (udd_and_1 f1 f2)) /\ (tpF (Sat f2) (udd_and_2 f1 f2)))) /\
-                                              (~ ((tpF (DisSat f1) (udd_and_3 f1 f2)) \/ (tpF (DisSat f2) (udd_and_4 f1 f2))))
-                 | ZF_Or f1 f2 => fun tpF => (~ ((tpF (Sat f1) (udd_or_1 f1 f2)) \/ (tpF (Sat f2) (udd_or_2 f1 f2)))) /\
-                                             (~ ((tpF (DisSat f1) (udd_or_3 f1 f2)) /\ (tpF (DisSat f2) (udd_or_4 f1 f2))))
-                 | ZF_Imp f1 f2 => fun tpF => (~ ((tpF (DisSat f1) (udd_imp_1 f1 f2)) \/ (tpF (Sat f2) (udd_imp_2 f1 f2)))) /\
-                                              (~ ((tpF (Sat f1) (udd_imp_3 f1 f2)) /\ (tpF (DisSat f2) (udd_imp_4 f1 f2))))
-                 | ZF_Not f => fun tpF => (~ ((tpF (DisSat f) (udd_not_1 f)))) /\ (~ ((tpF (Sat f) (udd_not_2 f))))
-                 | ZF_Forall v q f =>
-                   fun tpF => (~ (forall x : QT q, (tpF (Sat (substitute (v, @conv q x) f)) (udd_forall_1 f v q x)))) /\
-                              (~ (exists x : QT q, (tpF (DisSat (substitute (v, @conv q x) f)) (udd_forall_2 f v q x))))
-                 | ZF_Exists v q f =>
-                   fun tpF => (~ (exists x : QT q, (tpF (Sat (substitute (v, @conv q x) f)) (udd_exists_1 f v q x)))) /\
-                              (~ (forall x : QT q, (tpF (DisSat (substitute (v, @conv q x) f)) (udd_exists_2 f v q x))))
-               end
-           end).
-  Definition satisfied form := three_pred (Sat form).
-  Definition dissatisfied form := three_pred (DisSat form).
-  Definition undetermined form := three_pred (Undtmd form).
+    Definition three_pred : Input -> Prop :=
+      Fix inputOrder_wf (fun _ => Prop)
+          (fun (inp : Input) =>
+             match inp return ((forall ff : Input, inputOrder ff inp -> Prop) -> Prop) with
+               | Sat g =>
+                 match g with
+                   | ZF_BF bf      => fun _ => dzbf2bool bf = bool_inj true
+                   | ZF_And f1 f2  => fun tpF => (tpF (Sat f1) (sat_and_1 f1 f2)) /\ (tpF (Sat f2) (sat_and_2 f1 f2))
+                   | ZF_Or f1 f2   => fun tpF => (tpF (Sat f1) (sat_or_1 f1 f2)) \/ (tpF (Sat f2) (sat_or_2 f1 f2))
+                   | ZF_Imp f1 f2  => fun tpF => (tpF (DisSat f1) (sat_imp_1 f1 f2)) \/ (tpF (Sat f2) (sat_imp_2 f1 f2))
+                   | ZF_Not f      => fun tpF => (tpF (DisSat f) (sat_not f))
+                   | ZF_Forall v q f => fun tpF => forall x: QT q, (tpF (Sat (substitute (v, @conv q x) f)) (sat_forall f v q x))
+                   | ZF_Exists v q f => fun tpF => exists x: QT q, (tpF (Sat (substitute (v, @conv q x) f)) (sat_exists f v q x))
+                 end
+               | DisSat g =>
+                 match g with
+                   | ZF_BF bf => fun _ => dzbf2bool bf = bool_inj false
+                   | ZF_And f1 f2 => fun tpF => (tpF (DisSat f1) (dst_and_1 f1 f2)) \/ (tpF (DisSat f2) (dst_and_2 f1 f2))
+                   | ZF_Or f1 f2 => fun tpF => (tpF (DisSat f1) (dst_or_1 f1 f2)) /\ (tpF (DisSat f2) (dst_or_2 f1 f2))
+                   | ZF_Imp f1 f2 => fun tpF => (tpF (Sat f1) (dst_imp_1 f1 f2)) /\ (tpF (DisSat f2) (dst_imp_2 f1 f2))
+                   | ZF_Not f => fun tpF => (tpF (Sat f) (dst_not f))
+                   | ZF_Forall v q f => fun tpF => exists x : QT q,
+                                                     (tpF (DisSat (substitute (v, @conv q x) f)) (dst_forall f v q x))
+                   | ZF_Exists v q f => fun tpF => forall x : QT q,
+                                                     (tpF (DisSat (substitute (v, @conv q x) f)) (dst_exists f v q x))
+                 end
+               | Udtmd g =>
+                 match g with
+                   | ZF_BF bf => fun _ => (dzbf2bool bf <> bool_inj true) /\ (dzbf2bool bf <> bool_inj false)
+                   | ZF_And f1 f2 => fun tpF => (~ ((tpF (Sat f1) (udd_and_1 f1 f2)) /\ (tpF (Sat f2) (udd_and_2 f1 f2)))) /\
+                                                (~ ((tpF (DisSat f1) (udd_and_3 f1 f2)) \/ (tpF (DisSat f2) (udd_and_4 f1 f2))))
+                   | ZF_Or f1 f2 => fun tpF => (~ ((tpF (Sat f1) (udd_or_1 f1 f2)) \/ (tpF (Sat f2) (udd_or_2 f1 f2)))) /\
+                                               (~ ((tpF (DisSat f1) (udd_or_3 f1 f2)) /\ (tpF (DisSat f2) (udd_or_4 f1 f2))))
+                   | ZF_Imp f1 f2 => fun tpF => (~ ((tpF (DisSat f1) (udd_imp_1 f1 f2)) \/ (tpF (Sat f2) (udd_imp_2 f1 f2)))) /\
+                                                (~ ((tpF (Sat f1) (udd_imp_3 f1 f2)) /\ (tpF (DisSat f2) (udd_imp_4 f1 f2))))
+                   | ZF_Not f => fun tpF => (~ ((tpF (DisSat f) (udd_not_1 f)))) /\ (~ ((tpF (Sat f) (udd_not_2 f))))
+                   | ZF_Forall v q f =>
+                     fun tpF => (~ (forall x : QT q, (tpF (Sat (substitute (v, @conv q x) f)) (udd_forall_1 f v q x)))) /\
+                                (~ (exists x : QT q, (tpF (DisSat (substitute (v, @conv q x) f)) (udd_forall_2 f v q x))))
+                   | ZF_Exists v q f =>
+                     fun tpF => (~ (exists x : QT q, (tpF (Sat (substitute (v, @conv q x) f)) (udd_exists_1 f v q x)))) /\
+                                (~ (forall x : QT q, (tpF (DisSat (substitute (v, @conv q x) f)) (udd_exists_2 f v q x))))
+                 end
+             end).
+    Definition satisfied form := three_pred (Sat form).
+    Definition dissatisfied form := three_pred (DisSat form).
+    Definition undetermined form := three_pred (Udtmd form).
 
-  Lemma satisfied_unfold :
-    forall zf, satisfied zf = match zf with
-                                | ZF_BF bf      => (dzbf2bool bf = bool_inj true)
-                                | ZF_And f1 f2  => (satisfied f1) /\ (satisfied f2)
-                                | ZF_Or f1 f2   => (satisfied f1) \/ (satisfied f2)
-                                | ZF_Imp f1 f2  => (dissatisfied f1) \/ (satisfied f2)
-                                | ZF_Not f      =>  dissatisfied f
-                                | ZF_Forall v q f => forall x : QT q, (satisfied (substitute (v , @conv q x) f))
-                                | ZF_Exists v q f => exists x : QT q, (satisfied (substitute (v , @conv q x) f))
-                              end.
-  Proof.
-    intro; unfold satisfied at 1; unfold three_pred; rewrite Fix_eq;
-    [destruct zf | intros; assert (HFunEq: f = g) by (extensionality as1; extensionality as2; auto); subst; destruct x]; auto.
-  Qed.
+    Lemma satisfied_unfold :
+      forall zf, satisfied zf = match zf with
+                                  | ZF_BF bf      => (dzbf2bool bf = bool_inj true)
+                                  | ZF_And f1 f2  => (satisfied f1) /\ (satisfied f2)
+                                  | ZF_Or f1 f2   => (satisfied f1) \/ (satisfied f2)
+                                  | ZF_Imp f1 f2  => (dissatisfied f1) \/ (satisfied f2)
+                                  | ZF_Not f      =>  dissatisfied f
+                                  | ZF_Forall v q f => forall x : QT q, (satisfied (substitute (v , @conv q x) f))
+                                  | ZF_Exists v q f => exists x : QT q, (satisfied (substitute (v , @conv q x) f))
+                                end.
+    Proof.
+      intro; unfold satisfied at 1; unfold three_pred; rewrite Fix_eq;
+      [destruct zf | intros; assert (HFunEq: f = g) by (extensionality as1; extensionality as2; auto); subst; destruct x]; auto.
+    Qed.
 
-  Lemma dissatisfied_unfold :
-    forall zf, dissatisfied zf = match zf with
-                                   | ZF_BF bf      => (dzbf2bool bf = bool_inj false)
-                                   | ZF_And f1 f2  => (dissatisfied f1) \/ (dissatisfied f2)
-                                   | ZF_Or f1 f2   => (dissatisfied f1) /\ (dissatisfied f2)
-                                   | ZF_Imp f1 f2  => (satisfied f1) /\ (dissatisfied f2)
-                                   | ZF_Not f      => satisfied f
-                                   | ZF_Forall v q f => exists x : QT q, (dissatisfied (substitute (v , @conv q x) f))
-                                   | ZF_Exists v q f => forall x : QT q, (dissatisfied (substitute (v , @conv q x) f))
-                                 end.
-  Proof.
-    intro; unfold dissatisfied at 1; unfold three_pred; rewrite Fix_eq;
-    [destruct zf | intros; assert (HFunEq: f = g) by (extensionality as1; extensionality as2; auto); subst; destruct x]; auto.
-  Qed.
+    Lemma dissatisfied_unfold :
+      forall zf, dissatisfied zf = match zf with
+                                     | ZF_BF bf      => (dzbf2bool bf = bool_inj false)
+                                     | ZF_And f1 f2  => (dissatisfied f1) \/ (dissatisfied f2)
+                                     | ZF_Or f1 f2   => (dissatisfied f1) /\ (dissatisfied f2)
+                                     | ZF_Imp f1 f2  => (satisfied f1) /\ (dissatisfied f2)
+                                     | ZF_Not f      => satisfied f
+                                     | ZF_Forall v q f => exists x : QT q, (dissatisfied (substitute (v , @conv q x) f))
+                                     | ZF_Exists v q f => forall x : QT q, (dissatisfied (substitute (v , @conv q x) f))
+                                   end.
+    Proof.
+      intro; unfold dissatisfied at 1; unfold three_pred; rewrite Fix_eq;
+      [destruct zf | intros; assert (HFunEq: f = g) by (extensionality as1; extensionality as2; auto); subst; destruct x]; auto.
+    Qed.
 
-  Lemma undetermined_unfold : forall zf, undetermined zf <-> (~ satisfied zf) /\ (~ dissatisfied zf).
-  Proof.
-    intro; unfold undetermined at 1; unfold three_pred; rewrite satisfied_unfold, dissatisfied_unfold, Fix_eq;
-    [destruct zf | intros; assert (HFunEq: f = g) by (extensionality a; extensionality b; auto); subst; destruct x]; intuition.
-  Qed.
+    Lemma undetermined_unfold : forall zf, undetermined zf <-> (~ satisfied zf) /\ (~ dissatisfied zf).
+    Proof.
+      intro; unfold undetermined at 1; unfold three_pred; rewrite satisfied_unfold, dissatisfied_unfold, Fix_eq;
+      [destruct zf | intros; assert (HFunEq: f = g) by (extensionality a; extensionality b; auto); subst; destruct x]; intuition.
+    Qed.
 
-  Lemma sat_dissat_disj: forall zf, ~ (satisfied zf /\ dissatisfied zf).
-  Proof.
-    intro zf; remember (length_zform zf); assert (length_zform zf <= n) by omega; clear Heqn; revert zf H.
-    induction n; intros.
-    exfalso; destruct zf; simpl in H; intuition.
-    destruct zf; rewrite satisfied_unfold, dissatisfied_unfold; intro SS; destruct SS; simpl in H.
-    generalize bool_inj_not_eq; intro S; rewrite <- H0, <- H1 in S; apply S; trivial.
-    destruct H0; destruct H1; [apply (IHn zf1) | apply (IHn zf2)]; intuition.
-    destruct H1; destruct H0; [apply (IHn zf1) | apply (IHn zf2)]; intuition.
-    rewrite <- dissatisfied_unfold in H0; rewrite dissatisfied_unfold in H1.
-    destruct H1; destruct H0; [apply (IHn zf1) | apply (IHn zf2)]; intuition.
-    rewrite <- dissatisfied_unfold in H0; rewrite dissatisfied_unfold in H1; apply (IHn zf); intuition.
-    destruct H1; specialize (H0 x); apply (IHn (substitute (v, conv q x) zf)); [rewrite <- substitute_length_inv|]; intuition.
-    destruct H0; specialize (H1 x); apply (IHn (substitute (v, conv q x) zf)); [rewrite <- substitute_length_inv|]; intuition.
-  Qed.
+    Lemma sat_dissat_disj: forall zf, ~ (satisfied zf /\ dissatisfied zf).
+    Proof.
+      intro zf; remember (length_zform zf); assert (length_zform zf <= n) by omega; clear Heqn; revert zf H.
+      induction n; intros.
+      exfalso; destruct zf; simpl in H; intuition.
+      destruct zf; rewrite satisfied_unfold, dissatisfied_unfold; intro SS; destruct SS; simpl in H.
+      generalize bool_inj_not_eq; intro S; rewrite <- H0, <- H1 in S; apply S; trivial.
+      destruct H0; destruct H1; [apply (IHn zf1) | apply (IHn zf2)]; intuition.
+      destruct H1; destruct H0; [apply (IHn zf1) | apply (IHn zf2)]; intuition.
+      rewrite <- dissatisfied_unfold in H0; rewrite dissatisfied_unfold in H1.
+      destruct H1; destruct H0; [apply (IHn zf1) | apply (IHn zf2)]; intuition.
+      rewrite <- dissatisfied_unfold in H0; rewrite dissatisfied_unfold in H1; apply (IHn zf); intuition.
+      destruct H1; specialize (H0 x); apply (IHn (substitute (v, conv q x) zf)); [rewrite <- substitute_length_inv|]; intuition.
+      destruct H0; specialize (H1 x); apply (IHn (substitute (v, conv q x) zf)); [rewrite <- substitute_length_inv|]; intuition.
+    Qed.
 
-  Lemma sat_undtmd_disj : forall zf, ~ (satisfied zf /\ undetermined zf).
-  Proof. repeat intro; destruct H; rewrite undetermined_unfold in H0; destruct H0; apply H0; trivial. Qed.
+    Lemma sat_undtmd_disj : forall zf, ~ (satisfied zf /\ undetermined zf).
+    Proof. repeat intro; destruct H; rewrite undetermined_unfold in H0; destruct H0; apply H0; trivial. Qed.
 
-  Lemma dissat_undtmd_disj : forall zf, ~ (dissatisfied zf /\ undetermined zf).
-  Proof. repeat intro; destruct H; rewrite undetermined_unfold in H0; destruct H0; apply H1; trivial. Qed.
+    Lemma dissat_undtmd_disj : forall zf, ~ (dissatisfied zf /\ undetermined zf).
+    Proof. repeat intro; destruct H; rewrite undetermined_unfold in H0; destruct H0; apply H1; trivial. Qed.
 
-  Eval compute in satisfied (ZF_BF (ZBF_Const (bool_inj false))).
+    Eval compute in satisfied (ZF_BF (ZBF_Const (bool_inj false))).
 
-  Eval compute in satisfied (ZF_Or (ZF_BF (ZBF_Const (bool_inj true))) (ZF_BF (ZBF_Const (bool_inj false)))).
+    Eval compute in satisfied (ZF_Or (ZF_BF (ZBF_Const (bool_inj true))) (ZF_BF (ZBF_Const (bool_inj false)))).
 
-End DirectSemantics.
+  End DirectSemantics.
 
-Section ZFWellFounded.
+  Section ZFWellFounded.
 
-  Definition lengthOrder (f1 f2 : ZF) := length_zform f1 < length_zform f2.
+    Definition lengthOrder (f1 f2 : ZF) := length_zform f1 < length_zform f2.
 
-  Lemma lengthOrder_wf': forall len f, length_zform f <= len -> Acc lengthOrder f.
-  Proof.
-    induction len; intros; destruct f;
-    simpl in * |-; try omega;
-    constructor; intros; unfold lengthOrder in * |-; simpl in * |-;
-    apply IHlen with (f := y); omega.
-  Defined.
+    Lemma lengthOrder_wf': forall len f, length_zform f <= len -> Acc lengthOrder f.
+    Proof.
+      induction len; intros; destruct f;
+      simpl in * |-; try omega;
+      constructor; intros; unfold lengthOrder in * |-; simpl in * |-;
+                                                                    apply IHlen with (f := y); omega.
+    Defined.
 
-  Theorem lengthOrder_wf: well_founded lengthOrder.
-  Proof.
-    red; intro; eapply lengthOrder_wf'; eauto.
-  Defined.
+    Theorem lengthOrder_wf: well_founded lengthOrder.
+    Proof.
+      red; intro; eapply lengthOrder_wf'; eauto.
+    Defined.
 
-  Ltac smash := intros; unfold lengthOrder; simpl; omega || rewrite <- substitute_length_inv; omega.
+    Ltac smash := intros; unfold lengthOrder; simpl; omega || rewrite <- substitute_length_inv; omega.
 
-  Lemma lengthOrder_forall:forall f v q (x: QT q), lengthOrder (substitute (v, @conv q x) f) (ZF_Forall v q f). smash. Defined.
-  Lemma lengthOrder_forall_trivial: forall f v q, lengthOrder f (ZF_Forall v q f). smash. Defined.
-  Lemma lengthOrder_exists:forall f v q (x: QT q), lengthOrder (substitute (v, @conv q x) f) (ZF_Exists v q f). smash. Defined.
-  Lemma lengthOrder_exists_trivial: forall f v q, lengthOrder f (ZF_Exists v q f). smash. Defined.
-  Lemma lengthOrder_and_1: forall f1 f2, lengthOrder f1 (ZF_And f1 f2). smash. Defined.
-  Lemma lengthOrder_and_2: forall f1 f2, lengthOrder f2 (ZF_And f1 f2). smash. Defined.
-  Lemma lengthOrder_or_1: forall f1 f2, lengthOrder f1 (ZF_Or f1 f2). smash. Defined.
-  Lemma lengthOrder_or_2: forall f1 f2, lengthOrder f2 (ZF_Or f1 f2). smash. Defined.
-  Lemma lengthOrder_imp_1: forall f1 f2, lengthOrder f1 (ZF_Imp f1 f2). smash. Defined.
-  Lemma lengthOrder_imp_2: forall f1 f2, lengthOrder f2 (ZF_Imp f1 f2). smash. Defined.
-  Lemma lengthOrder_not: forall f, lengthOrder f (ZF_Not f). smash. Defined.
+    Lemma lengthOrder_forall:forall f v q (x: QT q), lengthOrder (substitute (v, @conv q x) f) (ZF_Forall v q f). smash. Defined.
+    Lemma lengthOrder_forall_trivial: forall f v q, lengthOrder f (ZF_Forall v q f). smash. Defined.
+    Lemma lengthOrder_exists:forall f v q (x: QT q), lengthOrder (substitute (v, @conv q x) f) (ZF_Exists v q f). smash. Defined.
+    Lemma lengthOrder_exists_trivial: forall f v q, lengthOrder f (ZF_Exists v q f). smash. Defined.
+    Lemma lengthOrder_and_1: forall f1 f2, lengthOrder f1 (ZF_And f1 f2). smash. Defined.
+    Lemma lengthOrder_and_2: forall f1 f2, lengthOrder f2 (ZF_And f1 f2). smash. Defined.
+    Lemma lengthOrder_or_1: forall f1 f2, lengthOrder f1 (ZF_Or f1 f2). smash. Defined.
+    Lemma lengthOrder_or_2: forall f1 f2, lengthOrder f2 (ZF_Or f1 f2). smash. Defined.
+    Lemma lengthOrder_imp_1: forall f1 f2, lengthOrder f1 (ZF_Imp f1 f2). smash. Defined.
+    Lemma lengthOrder_imp_2: forall f1 f2, lengthOrder f2 (ZF_Imp f1 f2). smash. Defined.
+    Lemma lengthOrder_not: forall f, lengthOrder f (ZF_Not f). smash. Defined.
 
-End ZFWellFounded.
+  End ZFWellFounded.
 
-Section Simplification.
+  Section Simplification.
 
-  (* Elimination of Min and Max *)
-  Definition eliminateMinMax (bf : ZBF) : ZF :=
-    match bf with
-        ZBF_Eq_Max e1 e2 e3 => ZF_Or (ZF_And (ZF_BF (ZBF_Eq e1 e2)) (ZF_BF (ZBF_Lte e3 e2)))
-                                     (ZF_And (ZF_BF (ZBF_Eq e1 e3)) (ZF_BF (ZBF_Lte e2 e3)))
-      | ZBF_Eq_Min e1 e2 e3 => ZF_Or (ZF_And (ZF_BF (ZBF_Eq e1 e2)) (ZF_BF (ZBF_Lte e2 e3)))
-                                     (ZF_And (ZF_BF (ZBF_Eq e1 e3)) (ZF_BF (ZBF_Lte e3 e2)))
-      | _ => ZF_BF bf
-    end.
+    (* Elimination of Min and Max *)
+    Definition eliminateMinMax (bf : ZBF) : ZF :=
+      match bf with
+          ZBF_Eq_Max e1 e2 e3 => ZF_Or (ZF_And (ZF_BF (ZBF_Eq e1 e2)) (ZF_BF (ZBF_Lte e3 e2)))
+                                       (ZF_And (ZF_BF (ZBF_Eq e1 e3)) (ZF_BF (ZBF_Lte e2 e3)))
+        | ZBF_Eq_Min e1 e2 e3 => ZF_Or (ZF_And (ZF_BF (ZBF_Eq e1 e2)) (ZF_BF (ZBF_Lte e2 e3)))
+                                       (ZF_And (ZF_BF (ZBF_Eq e1 e3)) (ZF_BF (ZBF_Lte e3 e2)))
+        | _ => ZF_BF bf
+      end.
 
-  (* Elimination of min and max doesn't change the validity of boolean forms *)
-  Lemma eliminate_ok: forall bf, satisfied (ZF_BF bf) <-> satisfied (eliminateMinMax bf).
-  Proof.
-    destruct bf; simpl; try tauto;
-    repeat rewrite satisfied_unfold;
-    simpl; rewrite truth_or_true_iff; repeat rewrite truth_and_true_iff; tauto.
-  Qed.
+    (* Elimination of min and max doesn't change the validity of boolean forms *)
+    Lemma eliminate_ok: forall bf, satisfied (ZF_BF bf) <-> satisfied (eliminateMinMax bf).
+    Proof.
+      destruct bf; simpl; try tauto;
+      repeat rewrite satisfied_unfold;
+      simpl; rewrite truth_or_true_iff; repeat rewrite truth_and_true_iff; tauto.
+    Qed.
 
-End Simplification.
+  End Simplification.
 
 End ArithSemantics.
