Transformation.v
@@ -35,295 +35,590 @@ Module InfSolver (sv:STRVAR) (VAL : SEM_VAL) (S: NONE_RELATION VAL).
   (* Variable domain is integers and constant domain is integers with infinity. *)
   Module I2F := ArithSemantics IntToInfinity sv VAL S InfRel.
 
-  (* Transform expressions in IA to I2F *)
-  Fixpoint inf_trans_exp (exp : IA.ZExp) : I2F.ZExp :=
-    match exp with
-        IA.ZExp_Var v => I2F.ZExp_Var v
-      | IA.ZExp_Const a => I2F.ZExp_Const a
-      | IA.ZExp_Add e1 e2 => I2F.ZExp_Add (inf_trans_exp e1) (inf_trans_exp e2)
-      | IA.ZExp_Inv e => I2F.ZExp_Inv (inf_trans_exp e)
-      | IA.ZExp_Sub e1 e2 => I2F.ZExp_Sub (inf_trans_exp e1) (inf_trans_exp e2)
-      | IA.ZExp_Mult z e => I2F.ZExp_Mult z (inf_trans_exp e)
-    end.
+  Section InfinityTransformation.
 
-  (* Expression transformation keeps the evaluation. *)
-  Lemma inf_trans_exp_ok : forall exp, IA.dexp2ZE exp = I2F.dexp2ZE (inf_trans_exp exp).
-  Proof.
-    induction exp; simpl; auto;
-    try (rewrite IHexp1, IHexp2; auto);
-    try (rewrite IHexp; auto).
-  Qed.
+    (* Transform expressions in IA to I2F *)
+    Fixpoint inf_trans_exp (exp : IA.ZExp) : I2F.ZExp :=
+      match exp with
+          IA.ZExp_Var v => I2F.ZExp_Var v
+        | IA.ZExp_Const a => I2F.ZExp_Const a
+        | IA.ZExp_Add e1 e2 => I2F.ZExp_Add (inf_trans_exp e1) (inf_trans_exp e2)
+        | IA.ZExp_Inv e => I2F.ZExp_Inv (inf_trans_exp e)
+        | IA.ZExp_Sub e1 e2 => I2F.ZExp_Sub (inf_trans_exp e1) (inf_trans_exp e2)
+        | IA.ZExp_Mult z e => I2F.ZExp_Mult z (inf_trans_exp e)
+      end.
 
-  (* Transform boolean forms in IA to I2F *)
-  Definition inf_trans_bf (bf : IA.ZBF) : I2F.ZBF :=
-    match bf with
-        IA.ZBF_Const b => I2F.ZBF_Const b
-      | IA.ZBF_Lt f1 f2 => I2F.ZBF_Lt (inf_trans_exp f1) (inf_trans_exp f2)
-      | IA.ZBF_Lte f1 f2 => I2F.ZBF_Lte (inf_trans_exp f1) (inf_trans_exp f2)
-      | IA.ZBF_Gt f1 f2 => I2F.ZBF_Gt (inf_trans_exp f1) (inf_trans_exp f2)
-      | IA.ZBF_Gte f1 f2 => I2F.ZBF_Gte (inf_trans_exp f1) (inf_trans_exp f2)
-      | IA.ZBF_Eq f1 f2 => I2F.ZBF_Eq (inf_trans_exp f1) (inf_trans_exp f2)
-      | IA.ZBF_Eq_Max f1 f2 f3 => I2F.ZBF_Eq_Max (inf_trans_exp f1) (inf_trans_exp f2) (inf_trans_exp f3)
-      | IA.ZBF_Eq_Min f1 f2 f3 => I2F.ZBF_Eq_Min (inf_trans_exp f1) (inf_trans_exp f2) (inf_trans_exp f3)
-      | IA.ZBF_Neq f1 f2 => I2F.ZBF_Neq (inf_trans_exp f1) (inf_trans_exp f2)
-    end.
+    (* Expression transformation keeps the evaluation. *)
+    Lemma inf_trans_exp_ok : forall exp, IA.dexp2ZE exp = I2F.dexp2ZE (inf_trans_exp exp).
+    Proof.
+      induction exp; simpl; auto;
+      try (rewrite IHexp1, IHexp2; auto);
+      try (rewrite IHexp; auto).
+    Qed.
 
-  (* Boolean form transformation keeps the validity. *)
-  Lemma inf_trans_bf_ok : forall z, IA.satisfied (IA.ZF_BF z) <-> I2F.satisfied (I2F.ZF_BF (inf_trans_bf z)).
-  Proof.
-    destruct z; simpl;
-    rewrite IA.satisfied_unfold, I2F.satisfied_unfold;
-    simpl; repeat rewrite inf_trans_exp_ok; tauto.
-  Qed.
+    (* Transform boolean forms in IA to I2F *)
+    Definition inf_trans_bf (bf : IA.ZBF) : I2F.ZBF :=
+      match bf with
+          IA.ZBF_Const b => I2F.ZBF_Const b
+        | IA.ZBF_Lt f1 f2 => I2F.ZBF_Lt (inf_trans_exp f1) (inf_trans_exp f2)
+        | IA.ZBF_Lte f1 f2 => I2F.ZBF_Lte (inf_trans_exp f1) (inf_trans_exp f2)
+        | IA.ZBF_Gt f1 f2 => I2F.ZBF_Gt (inf_trans_exp f1) (inf_trans_exp f2)
+        | IA.ZBF_Gte f1 f2 => I2F.ZBF_Gte (inf_trans_exp f1) (inf_trans_exp f2)
+        | IA.ZBF_Eq f1 f2 => I2F.ZBF_Eq (inf_trans_exp f1) (inf_trans_exp f2)
+        | IA.ZBF_Eq_Max f1 f2 f3 => I2F.ZBF_Eq_Max (inf_trans_exp f1) (inf_trans_exp f2) (inf_trans_exp f3)
+        | IA.ZBF_Eq_Min f1 f2 f3 => I2F.ZBF_Eq_Min (inf_trans_exp f1) (inf_trans_exp f2) (inf_trans_exp f3)
+        | IA.ZBF_Neq f1 f2 => I2F.ZBF_Neq (inf_trans_exp f1) (inf_trans_exp f2)
+      end.
 
-  Lemma inf_trans_bf_dst : forall z, IA.dissatisfied (IA.ZF_BF z) <-> I2F.dissatisfied (I2F.ZF_BF (inf_trans_bf z)).
-  Proof.
-    destruct z; simpl;
-    rewrite IA.dissatisfied_unfold, I2F.dissatisfied_unfold;
-    simpl; repeat rewrite inf_trans_exp_ok; tauto.
-  Qed.
+    (* Boolean form transformation keeps the validity. *)
+    Lemma inf_trans_bf_ok : forall z, IA.satisfied (IA.ZF_BF z) <-> I2F.satisfied (I2F.ZF_BF (inf_trans_bf z)).
+    Proof.
+      destruct z; simpl;
+      rewrite IA.satisfied_unfold, I2F.satisfied_unfold;
+      simpl; repeat rewrite inf_trans_exp_ok; tauto.
+    Qed.
 
-  (* Transform logic forms in IA to I2F *)
-  Definition inf_trans : IA.ZF -> I2F.ZF :=
-    Fix IA.lengthOrder_wf (fun _ => I2F.ZF)
-        (fun (form : IA.ZF) =>
-           match form return ((forall f : IA.ZF, IA.lengthOrder f form -> I2F.ZF) -> I2F.ZF) with
-               IA.ZF_BF bf => fun _ => I2F.ZF_BF (inf_trans_bf bf)
-             | IA.ZF_And f1 f2 => fun infTrans => I2F.ZF_And (infTrans f1 (IA.lengthOrder_and_1 f1 f2))
-                                                             (infTrans f2 (IA.lengthOrder_and_2 f1 f2))
-             | IA.ZF_Or f1 f2 => fun infTrans => I2F.ZF_Or (infTrans f1 (IA.lengthOrder_or_1 f1 f2))
-                                                           (infTrans f2 (IA.lengthOrder_or_2 f1 f2))
-             | IA.ZF_Imp f1 f2 => fun infTrans => I2F.ZF_Imp (infTrans f1 (IA.lengthOrder_imp_1 f1 f2))
-                                                             (infTrans f2 (IA.lengthOrder_imp_2 f1 f2))
-             | IA.ZF_Not f' => fun infTrans => I2F.ZF_Not (infTrans f' (IA.lengthOrder_not f'))
-             | IA.ZF_Forall v q f' =>
-               match q with
-                   PureInfinity.Q_Z =>
-                   fun infTrans => I2F.ZF_Forall v tt (infTrans f' (IA.lengthOrder_forall_trivial f' v PureInfinity.Q_Z))
-                 | PureInfinity.Q_ZE =>
-                   fun infTrans =>
-                     I2F.ZF_And (I2F.ZF_Forall v tt (infTrans f' (IA.lengthOrder_forall_trivial f' v PureInfinity.Q_ZE)))
-                                (I2F.ZF_And (infTrans (IA.substitute (v, Some ZE_Inf) f')
-                                                      (IA.lengthOrder_forall f' v PureInfinity.Q_ZE ZE_Inf))
+    Lemma inf_trans_bf_dst : forall z, IA.dissatisfied (IA.ZF_BF z) <-> I2F.dissatisfied (I2F.ZF_BF (inf_trans_bf z)).
+    Proof.
+      destruct z; simpl;
+      rewrite IA.dissatisfied_unfold, I2F.dissatisfied_unfold;
+      simpl; repeat rewrite inf_trans_exp_ok; tauto.
+    Qed.
+
+    (* Transform logic forms in IA to I2F *)
+    Definition inf_trans : IA.ZF -> I2F.ZF :=
+      Fix IA.lengthOrder_wf (fun _ => I2F.ZF)
+          (fun (form : IA.ZF) =>
+             match form return ((forall f : IA.ZF, IA.lengthOrder f form -> I2F.ZF) -> I2F.ZF) with
+                 IA.ZF_BF bf => fun _ => I2F.ZF_BF (inf_trans_bf bf)
+               | IA.ZF_And f1 f2 => fun infTrans => I2F.ZF_And (infTrans f1 (IA.lengthOrder_and_1 f1 f2))
+                                                               (infTrans f2 (IA.lengthOrder_and_2 f1 f2))
+               | IA.ZF_Or f1 f2 => fun infTrans => I2F.ZF_Or (infTrans f1 (IA.lengthOrder_or_1 f1 f2))
+                                                             (infTrans f2 (IA.lengthOrder_or_2 f1 f2))
+               | IA.ZF_Imp f1 f2 => fun infTrans => I2F.ZF_Imp (infTrans f1 (IA.lengthOrder_imp_1 f1 f2))
+                                                               (infTrans f2 (IA.lengthOrder_imp_2 f1 f2))
+               | IA.ZF_Not f' => fun infTrans => I2F.ZF_Not (infTrans f' (IA.lengthOrder_not f'))
+               | IA.ZF_Forall v q f' =>
+                 match q with
+                     PureInfinity.Q_Z =>
+                     fun infTrans => I2F.ZF_Forall v tt (infTrans f' (IA.lengthOrder_forall_trivial f' v PureInfinity.Q_Z))
+                   | PureInfinity.Q_ZE =>
+                     fun infTrans =>
+                       I2F.ZF_And (I2F.ZF_Forall v tt (infTrans f' (IA.lengthOrder_forall_trivial f' v PureInfinity.Q_ZE)))
+                                  (I2F.ZF_And (infTrans (IA.substitute (v, Some ZE_Inf) f')
+                                                        (IA.lengthOrder_forall f' v PureInfinity.Q_ZE ZE_Inf))
+                                              (infTrans (IA.substitute (v, Some ZE_NegInf) f')
+                                                        (IA.lengthOrder_forall f' v PureInfinity.Q_ZE ZE_NegInf)))
+                 end
+               | IA.ZF_Exists v q f' =>
+                 match q with
+                     PureInfinity.Q_Z =>
+                     fun infTrans => I2F.ZF_Exists v tt (infTrans f' (IA.lengthOrder_exists_trivial f' v PureInfinity.Q_Z))
+                   | PureInfinity.Q_ZE =>
+                     fun infTrans =>
+                       I2F.ZF_Or (I2F.ZF_Exists v tt (infTrans f' (IA.lengthOrder_exists_trivial f' v PureInfinity.Q_ZE)))
+                                 (I2F.ZF_Or (infTrans (IA.substitute (v, Some ZE_Inf) f')
+                                                      (IA.lengthOrder_exists f' v PureInfinity.Q_ZE ZE_Inf))
                                             (infTrans (IA.substitute (v, Some ZE_NegInf) f')
-                                                      (IA.lengthOrder_forall f' v PureInfinity.Q_ZE ZE_NegInf)))
-               end
-             | IA.ZF_Exists v q f' =>
-               match q with
-                   PureInfinity.Q_Z =>
-                   fun infTrans => I2F.ZF_Exists v tt (infTrans f' (IA.lengthOrder_exists_trivial f' v PureInfinity.Q_Z))
-                 | PureInfinity.Q_ZE =>
-                   fun infTrans =>
-                     I2F.ZF_Or (I2F.ZF_Exists v tt (infTrans f' (IA.lengthOrder_exists_trivial f' v PureInfinity.Q_ZE)))
-                               (I2F.ZF_Or (infTrans (IA.substitute (v, Some ZE_Inf) f')
-                                                    (IA.lengthOrder_exists f' v PureInfinity.Q_ZE ZE_Inf))
-                                          (infTrans (IA.substitute (v, Some ZE_NegInf) f')
-                                                    (IA.lengthOrder_exists f' v PureInfinity.Q_ZE ZE_NegInf)))
-               end
-           end).
+                                                      (IA.lengthOrder_exists f' v PureInfinity.Q_ZE ZE_NegInf)))
+                 end
+             end).
 
-  Lemma inf_trans_unfold: forall form,
-                            inf_trans form =
-                            match form with
-                                IA.ZF_BF bf => I2F.ZF_BF (inf_trans_bf bf)
-                              | IA.ZF_And f1 f2 => I2F.ZF_And (inf_trans f1) (inf_trans f2)
-                              | IA.ZF_Or f1 f2 => I2F.ZF_Or (inf_trans f1) (inf_trans f2)
-                              | IA.ZF_Imp f1 f2 => I2F.ZF_Imp (inf_trans f1) (inf_trans f2)
-                              | IA.ZF_Not f => I2F.ZF_Not (inf_trans f)
-                              | IA.ZF_Forall v q f =>
-                                match q with
-                                    PureInfinity.Q_Z => I2F.ZF_Forall v tt (inf_trans f)
-                                  | PureInfinity.Q_ZE => I2F.ZF_And (I2F.ZF_Forall v tt (inf_trans f))
-                                                                    (I2F.ZF_And (inf_trans (IA.substitute (v, Some ZE_Inf) f))
-                                                                                (inf_trans (IA.substitute (v, Some ZE_NegInf) f)))
-                                end
-                              | IA.ZF_Exists v q f =>
-                                match q with
-                                    PureInfinity.Q_Z => I2F.ZF_Exists v tt (inf_trans f)
-                                  | PureInfinity.Q_ZE => I2F.ZF_Or (I2F.ZF_Exists v tt (inf_trans f))
-                                                                   (I2F.ZF_Or (inf_trans (IA.substitute (v, Some ZE_Inf) f))
-                                                                              (inf_trans (IA.substitute (v, Some ZE_NegInf) f)))
-                                end
-                            end.
-  Proof.
-    intro; unfold inf_trans at 1; rewrite Fix_eq.
-    destruct form; auto;
-    destruct q; auto.
-    intros; match goal with
-              | [H : forall (y : IA.ZF) (p : IA.lengthOrder y ?x), ?f y p = ?g y p |- _ ] =>
-                assert (HFunEq: f = g) by (extensionality as1; extensionality as2; auto);
-                  destruct x; auto; repeat (f_equal; auto); rewrite HFunEq; reflexivity
-            end.
-  Qed.
+    Lemma inf_trans_unfold:
+      forall form,
+        inf_trans form =
+        match form with
+            IA.ZF_BF bf => I2F.ZF_BF (inf_trans_bf bf)
+          | IA.ZF_And f1 f2 => I2F.ZF_And (inf_trans f1) (inf_trans f2)
+          | IA.ZF_Or f1 f2 => I2F.ZF_Or (inf_trans f1) (inf_trans f2)
+          | IA.ZF_Imp f1 f2 => I2F.ZF_Imp (inf_trans f1) (inf_trans f2)
+          | IA.ZF_Not f => I2F.ZF_Not (inf_trans f)
+          | IA.ZF_Forall v q f =>
+            match q with
+                PureInfinity.Q_Z => I2F.ZF_Forall v tt (inf_trans f)
+              | PureInfinity.Q_ZE => I2F.ZF_And (I2F.ZF_Forall v tt (inf_trans f))
+                                                (I2F.ZF_And (inf_trans (IA.substitute (v, Some ZE_Inf) f))
+                                                            (inf_trans (IA.substitute (v, Some ZE_NegInf) f)))
+            end
+          | IA.ZF_Exists v q f =>
+            match q with
+                PureInfinity.Q_Z => I2F.ZF_Exists v tt (inf_trans f)
+              | PureInfinity.Q_ZE => I2F.ZF_Or (I2F.ZF_Exists v tt (inf_trans f))
+                                               (I2F.ZF_Or (inf_trans (IA.substitute (v, Some ZE_Inf) f))
+                                                          (inf_trans (IA.substitute (v, Some ZE_NegInf) f)))
+            end
+        end.
+    Proof.
+      intro; unfold inf_trans at 1; rewrite Fix_eq.
+      destruct form; auto;
+      destruct q; auto.
+      intros; match goal with
+                | [H : forall (y : IA.ZF) (p : IA.lengthOrder y ?x), ?f y p = ?g y p |- _ ] =>
+                  assert (HFunEq: f = g) by (extensionality as1; extensionality as2; auto);
+                    destruct x; auto; repeat (f_equal; auto); rewrite HFunEq; reflexivity
+              end.
+    Qed.
 
-  (* Substitution and expression transformation from IA to I2F are commutative. *)
-  Lemma subst_inf_trans_exp_eq : forall z v (x : option ZE),
-                                   I2F.subst_exp (v, x) (inf_trans_exp z) = inf_trans_exp (IA.subst_exp (v, x) z).
-  Proof.
-    induction z; simpl; intros;
-    try (destruct (var_eq_dec v0 v); simpl);
-    try (rewrite IHz1, IHz2);
-    try (rewrite IHz);
-    auto.
-  Qed.
+    (* Substitution and expression transformation from IA to I2F are commutative. *)
+    Lemma subst_inf_trans_exp_eq : forall z v (x : option ZE),
+                                     I2F.subst_exp (v, x) (inf_trans_exp z) = inf_trans_exp (IA.subst_exp (v, x) z).
+    Proof.
+      induction z; simpl; intros;
+      try (destruct (var_eq_dec v0 v); simpl);
+      try (rewrite IHz1, IHz2);
+      try (rewrite IHz);
+      auto.
+    Qed.
 
-  (* Substitution and boolean form transformation from IA to I2F are commutative. *)
-  Lemma subst_inf_trans_bf_eq : forall z v (x : option ZE),
-                                  I2F.substitute (v, x) (inf_trans (IA.ZF_BF z)) =
-                                  inf_trans (IA.substitute (v, x) (IA.ZF_BF z)).
-  Proof.
-    destruct z; simpl; intros;
-    unfold inf_trans;
-    unfold IA.length_zform;
-    simpl; auto;
-    repeat rewrite subst_inf_trans_exp_eq; auto.
-  Qed.
+    (* Substitution and boolean form transformation from IA to I2F are commutative. *)
+    Lemma subst_inf_trans_bf_eq : forall z v (x : option ZE),
+                                    I2F.substitute (v, x) (inf_trans (IA.ZF_BF z)) =
+                                    inf_trans (IA.substitute (v, x) (IA.ZF_BF z)).
+    Proof.
+      destruct z; simpl; intros;
+      unfold inf_trans;
+      unfold IA.length_zform;
+      simpl; auto;
+      repeat rewrite subst_inf_trans_exp_eq; auto.
+    Qed.
 
-  Ltac unfold_right_inf_trans :=
-    match goal with
-      | [|- _ = inf_trans ?X] => rewrite inf_trans_unfold with X; auto
-    end.
+    Ltac unfold_right_inf_trans :=
+      match goal with
+        | [|- _ = inf_trans ?X] => rewrite inf_trans_unfold with X; auto
+      end.
 
-  (* Substitution and logic form transformation from IA to I2F are commutative. *)
-  Lemma subst_inf_trans_eq: forall f v (x: option ZE), I2F.substitute (v, x) (inf_trans f) = inf_trans (IA.substitute (v, x) f).
-  Proof.
-    intros f; remember (IA.length_zform f); assert (IA.length_zform f <= n) by omega; clear Heqn; revert f H;
-    induction n; intros;
-    [ destruct f; exfalso; simpl in H; intuition |
-      destruct f; simpl in H; apply le_S_n in H;
-      let solve_cnt := (rewrite inf_trans_unfold; simpl; rewrite (IHn f1), (IHn f2);
-                        [unfold_right_inf_trans | omega | omega ]) in
-      let solve_quant :=
-          rewrite inf_trans_unfold; destruct q; simpl;
-          [destruct (var_eq_dec v v0); unfold_right_inf_trans; rewrite IHn; auto |
-           destruct (var_eq_dec v v0); repeat rewrite <- IHn; auto;
-           [rewrite e; repeat rewrite I2F.same_var_subst |
-            repeat rewrite I2F.diff_var_subst with (v1 := v) (v2 := v0); auto];
-           unfold_right_inf_trans; repeat rewrite IHn; auto; rewrite <- IA.substitute_length_inv; auto] in
-      solve [rewrite subst_inf_trans_bf_eq; auto | solve_cnt | solve_cnt | solve_cnt |
-             rewrite inf_trans_unfold; simpl; rewrite IHn; [unfold_right_inf_trans | omega ] |
-             solve_quant | solve_quant]].
-  Qed.
+    (* Substitution and logic form transformation from IA to I2F are commutative. *)
+    Lemma subst_inf_trans_eq: forall f v (x: option ZE), I2F.substitute (v, x) (inf_trans f) =
+                                                         inf_trans (IA.substitute (v, x) f).
+    Proof.
+      intros f; remember (IA.length_zform f); assert (IA.length_zform f <= n) by omega; clear Heqn; revert f H;
+      induction n; intros;
+      [ destruct f; exfalso; simpl in H; intuition |
+        destruct f; simpl in H; apply le_S_n in H;
+        let solve_cnt := (rewrite inf_trans_unfold; simpl; rewrite (IHn f1), (IHn f2);
+                          [unfold_right_inf_trans | omega | omega ]) in
+        let solve_quant :=
+            rewrite inf_trans_unfold; destruct q; simpl;
+            [destruct (var_eq_dec v v0); unfold_right_inf_trans; rewrite IHn; auto |
+             destruct (var_eq_dec v v0); repeat rewrite <- IHn; auto;
+             [rewrite e; repeat rewrite I2F.same_var_subst |
+              repeat rewrite I2F.diff_var_subst with (v1 := v) (v2 := v0); auto];
+             unfold_right_inf_trans; repeat rewrite IHn; auto; rewrite <- IA.substitute_length_inv; auto] in
+        solve [rewrite subst_inf_trans_bf_eq; auto | solve_cnt | solve_cnt | solve_cnt |
+               rewrite inf_trans_unfold; simpl; rewrite IHn; [unfold_right_inf_trans | omega ] |
+               solve_quant | solve_quant]].
+    Qed.
 
-  Ltac solve_le_inv :=
-    match goal with
-      | [|- IA.length_zform (IA.substitute _ _) <= _] => rewrite <- IA.substitute_length_inv; auto
-    end.
+    Ltac solve_le_inv :=
+      match goal with
+        | [|- IA.length_zform (IA.substitute _ _) <= _] => rewrite <- IA.substitute_length_inv; auto
+      end.
 
-  (* Logic form transformation from IA to I2F keeps the validity. *)
-  Lemma inf_trans_ok : forall f, (IA.satisfied f <-> I2F.satisfied (inf_trans f)) /\
-                                 (IA.dissatisfied f <-> I2F.dissatisfied (inf_trans f)).
-  Proof.
-    intros f; remember (IA.length_zform f); assert (IA.length_zform f <= n) by omega; clear Heqn; revert f H.
-    induction n; intros.
-    exfalso; destruct f; simpl in H; intuition.
-    split.
-    (* ok part *)
-    destruct f; simpl in H; apply le_S_n in H; rewrite inf_trans_unfold; try (rewrite inf_trans_bf_ok; intuition);
-    rewrite IA.satisfied_unfold, I2F.satisfied_unfold.
-    assert (S1: IA.length_zform f1 <= n) by omega; assert (S2: IA.length_zform f2 <= n) by omega;
-    destruct (IHn _ S1); destruct (IHn _ S2); intuition.
-    assert (S1: IA.length_zform f1 <= n) by omega; assert (S2: IA.length_zform f2 <= n) by omega;
-    destruct (IHn _ S1); destruct (IHn _ S2); intuition.
-    assert (S1: IA.length_zform f1 <= n) by omega; assert (S2: IA.length_zform f2 <= n) by omega;
-    destruct (IHn _ S1); destruct (IHn _ S2); intuition.
-    assert (S: IA.length_zform f <= n) by omega; destruct (IHn _ S); intuition.
+    (* Logic form transformation from IA to I2F keeps the validity. *)
+    Lemma inf_trans_ok : forall f, (IA.satisfied f <-> I2F.satisfied (inf_trans f)) /\
+                                   (IA.dissatisfied f <-> I2F.dissatisfied (inf_trans f)).
+    Proof.
+      intros f; remember (IA.length_zform f); assert (IA.length_zform f <= n) by omega; clear Heqn; revert f H.
+      induction n; intros.
+      exfalso; destruct f; simpl in H; intuition.
+      split.
+      (* ok part *)
+      destruct f; simpl in H; apply le_S_n in H; rewrite inf_trans_unfold; try (rewrite inf_trans_bf_ok; intuition);
+      rewrite IA.satisfied_unfold, I2F.satisfied_unfold.
+      assert (S1: IA.length_zform f1 <= n) by omega; assert (S2: IA.length_zform f2 <= n) by omega;
+      destruct (IHn _ S1); destruct (IHn _ S2); intuition.
+      assert (S1: IA.length_zform f1 <= n) by omega; assert (S2: IA.length_zform f2 <= n) by omega;
+      destruct (IHn _ S1); destruct (IHn _ S2); intuition.
+      assert (S1: IA.length_zform f1 <= n) by omega; assert (S2: IA.length_zform f2 <= n) by omega;
+      destruct (IHn _ S1); destruct (IHn _ S2); intuition.
+      assert (S: IA.length_zform f <= n) by omega; destruct (IHn _ S); intuition.
 
-    assert (INV1: IA.length_zform (IA.substitute (v,Some ZE_Inf) f) <= n) by solve_le_inv; destruct (IHn _ INV1) as [SAT1 DST1];
-    assert (INV2: IA.length_zform(IA.substitute(v,Some ZE_NegInf) f)<= n) by solve_le_inv; destruct (IHn _ INV2) as [SAT2 DST2].
-    destruct q; unfold PureInfinity.QT, IntToInfinity.QT.
-    split; intros; assert (INV: IA.length_zform (IA.substitute (v, @IntToInfinity.conv tt x) f) <= n) by solve_le_inv;
-    destruct (IHn _ INV) as [SAT DST];
-    [rewrite subst_inf_trans_eq; rewrite <- SAT | rewrite SAT; rewrite <- subst_inf_trans_eq]; apply H0.
-    do 2 rewrite I2F.satisfied_unfold; split; intros.
-    split; intros.
-    assert (INV: IA.length_zform (IA.substitute (v, @IntToInfinity.conv tt x) f) <= n) by solve_le_inv;
-    destruct (IHn _ INV) as [SAT DST].
-    rewrite subst_inf_trans_eq; rewrite <- SAT; apply H0.
-    split; [rewrite <- SAT1 | rewrite <- SAT2].
-    apply H0. apply H0. destruct H0 as [? [? ?]].
-    destruct x.
-    assert (INV: IA.length_zform (IA.substitute (v, @PureInfinity.conv PureInfinity.Q_Z z) f) <= n) by solve_le_inv;
-      destruct (IHn _ INV) as [SAT DST].
-    rewrite SAT; rewrite <- subst_inf_trans_eq; apply H0.
-    rewrite SAT1; apply H1. rewrite SAT2; apply H2.
+      assert (INV1: IA.length_zform (IA.substitute(v,Some ZE_Inf)f) <= n) by solve_le_inv; destruct (IHn _ INV1) as [SAT1 DST1];
+      assert (INV2: IA.length_zform(IA.substitute(v,Some ZE_NegInf)f)<=n) by solve_le_inv; destruct (IHn _ INV2) as [SAT2 DST2].
+      destruct q; unfold PureInfinity.QT, IntToInfinity.QT.
+      split; intros; assert (INV: IA.length_zform (IA.substitute (v, @IntToInfinity.conv tt x) f) <= n) by solve_le_inv;
+      destruct (IHn _ INV) as [SAT DST];
+      [rewrite subst_inf_trans_eq; rewrite <- SAT | rewrite SAT; rewrite <- subst_inf_trans_eq]; apply H0.
+      do 2 rewrite I2F.satisfied_unfold; split; intros.
+      split; intros.
+      assert (INV: IA.length_zform (IA.substitute (v, @IntToInfinity.conv tt x) f) <= n) by solve_le_inv;
+        destruct (IHn _ INV) as [SAT DST].
+      rewrite subst_inf_trans_eq; rewrite <- SAT; apply H0.
+      split; [rewrite <- SAT1 | rewrite <- SAT2].
+      apply H0. apply H0. destruct H0 as [? [? ?]].
+      destruct x.
+      assert (INV: IA.length_zform (IA.substitute (v, @PureInfinity.conv PureInfinity.Q_Z z) f) <= n) by solve_le_inv;
+        destruct (IHn _ INV) as [SAT DST].
+      rewrite SAT; rewrite <- subst_inf_trans_eq; apply H0.
+      rewrite SAT1; apply H1. rewrite SAT2; apply H2.
 
-    assert (INV1: IA.length_zform (IA.substitute (v,Some ZE_Inf) f) <= n) by solve_le_inv; destruct (IHn _ INV1) as [SAT1 DST1];
-    assert (INV2: IA.length_zform(IA.substitute(v,Some ZE_NegInf) f)<= n) by solve_le_inv; destruct (IHn _ INV2) as [SAT2 DST2].
-    destruct q; unfold PureInfinity.QT, IntToInfinity.QT.
-    split; intros; destruct H0 as [x H0]; exists x;
-    assert (INV: IA.length_zform (IA.substitute (v, @IntToInfinity.conv tt x) f) <= n) by solve_le_inv;
-    destruct (IHn _ INV) as [SAT DST];
-    [rewrite subst_inf_trans_eq; rewrite <- SAT | rewrite SAT; rewrite <- subst_inf_trans_eq]; apply H0.
-    do 2 rewrite I2F.satisfied_unfold; split; intros.
-    destruct H0 as [x H0]; destruct x.
-    left; exists z; rewrite subst_inf_trans_eq.
-    assert (INV: IA.length_zform (IA.substitute (v, @PureInfinity.conv PureInfinity.Q_Z z) f) <= n) by solve_le_inv;
-      destruct (IHn _ INV) as [SAT DST].
-    rewrite <- SAT; apply H0.
-    right; left; rewrite <- SAT1; apply H0.
-    right; right; rewrite <- SAT2; apply H0.
-    destruct H0; destruct H0.
-    exists (ZE_Fin x).
-    assert (INV: IA.length_zform (IA.substitute (v, @PureInfinity.conv PureInfinity.Q_ZE (ZE_Fin x)) f) <= n) by solve_le_inv;
-      destruct (IHn _ INV) as [SAT DST].
-    rewrite SAT; rewrite <- subst_inf_trans_eq; apply H0.
-    exists ZE_Inf; rewrite SAT1; apply H0.
-    exists ZE_NegInf; rewrite SAT2; apply H0.
+      assert (INV1: IA.length_zform (IA.substitute(v,Some ZE_Inf)f) <= n) by solve_le_inv; destruct (IHn _ INV1) as [SAT1 DST1];
+      assert (INV2: IA.length_zform(IA.substitute(v,Some ZE_NegInf)f)<=n) by solve_le_inv; destruct (IHn _ INV2) as [SAT2 DST2].
+      destruct q; unfold PureInfinity.QT, IntToInfinity.QT.
+      split; intros; destruct H0 as [x H0]; exists x;
+      assert (INV: IA.length_zform (IA.substitute (v, @IntToInfinity.conv tt x) f) <= n) by solve_le_inv;
+      destruct (IHn _ INV) as [SAT DST];
+      [rewrite subst_inf_trans_eq; rewrite <- SAT | rewrite SAT; rewrite <- subst_inf_trans_eq]; apply H0.
+      do 2 rewrite I2F.satisfied_unfold; split; intros.
+      destruct H0 as [x H0]; destruct x.
+      left; exists z; rewrite subst_inf_trans_eq.
+      assert (INV: IA.length_zform (IA.substitute (v, @PureInfinity.conv PureInfinity.Q_Z z) f) <= n) by solve_le_inv;
+        destruct (IHn _ INV) as [SAT DST].
+      rewrite <- SAT; apply H0.
+      right; left; rewrite <- SAT1; apply H0.
+      right; right; rewrite <- SAT2; apply H0.
+      destruct H0; destruct H0.
+      exists (ZE_Fin x).
+      assert (INV: IA.length_zform (IA.substitute (v, @PureInfinity.conv PureInfinity.Q_ZE (ZE_Fin x)) f) <= n) by solve_le_inv;
+        destruct (IHn _ INV) as [SAT DST].
+      rewrite SAT; rewrite <- subst_inf_trans_eq; apply H0.
+      exists ZE_Inf; rewrite SAT1; apply H0.
+      exists ZE_NegInf; rewrite SAT2; apply H0.
 
-    (* dst part *)
-    (* intros f; remember (IA.length_zform f); assert (IA.length_zform f <= n) by omega; clear Heqn; revert f H; *)
-    destruct f; simpl in H; apply le_S_n in H; rewrite inf_trans_unfold; try (rewrite inf_trans_bf_dst; intuition);
-    rewrite IA.dissatisfied_unfold, I2F.dissatisfied_unfold.
-    assert (S1: IA.length_zform f1 <= n) by omega; assert (S2: IA.length_zform f2 <= n) by omega;
-    destruct (IHn _ S1); destruct (IHn _ S2); intuition.
-    assert (S1: IA.length_zform f1 <= n) by omega; assert (S2: IA.length_zform f2 <= n) by omega;
-    destruct (IHn _ S1); destruct (IHn _ S2); intuition.
-    assert (S1: IA.length_zform f1 <= n) by omega; assert (S2: IA.length_zform f2 <= n) by omega;
-    destruct (IHn _ S1); destruct (IHn _ S2); intuition.
-    assert (S: IA.length_zform f <= n) by omega; destruct (IHn _ S); intuition.
+      (* dst part *)
+      (* intros f; remember (IA.length_zform f); assert (IA.length_zform f <= n) by omega; clear Heqn; revert f H; *)
+      destruct f; simpl in H; apply le_S_n in H; rewrite inf_trans_unfold; try (rewrite inf_trans_bf_dst; intuition);
+      rewrite IA.dissatisfied_unfold, I2F.dissatisfied_unfold.
+      assert (S1: IA.length_zform f1 <= n) by omega; assert (S2: IA.length_zform f2 <= n) by omega;
+      destruct (IHn _ S1); destruct (IHn _ S2); intuition.
+      assert (S1: IA.length_zform f1 <= n) by omega; assert (S2: IA.length_zform f2 <= n) by omega;
+      destruct (IHn _ S1); destruct (IHn _ S2); intuition.
+      assert (S1: IA.length_zform f1 <= n) by omega; assert (S2: IA.length_zform f2 <= n) by omega;
+      destruct (IHn _ S1); destruct (IHn _ S2); intuition.
+      assert (S: IA.length_zform f <= n) by omega; destruct (IHn _ S); intuition.
 
-    assert (INV1: IA.length_zform (IA.substitute (v,Some ZE_Inf) f) <= n) by solve_le_inv; destruct (IHn _ INV1) as [SAT1 DST1];
-    assert (INV2: IA.length_zform(IA.substitute(v,Some ZE_NegInf) f)<= n) by solve_le_inv; destruct (IHn _ INV2) as [SAT2 DST2].
-    destruct q; unfold PureInfinity.QT, IntToInfinity.QT.
-    split; intros; destruct H0 as [x H0]; exists x;
-    assert (INV: IA.length_zform (IA.substitute (v, @IntToInfinity.conv tt x) f) <= n) by solve_le_inv;
-    destruct (IHn _ INV) as [SAT DST];
-    [rewrite subst_inf_trans_eq; rewrite <- DST | rewrite DST; rewrite <- subst_inf_trans_eq]; apply H0.
-    do 2 rewrite I2F.dissatisfied_unfold; split; intros.
-    destruct H0 as [x H0]; destruct x.
-    left; exists z; rewrite subst_inf_trans_eq.
-    assert (INV: IA.length_zform (IA.substitute (v, @PureInfinity.conv PureInfinity.Q_Z z) f) <= n) by solve_le_inv;
-      destruct (IHn _ INV) as [SAT DST].
-    rewrite <- DST; apply H0.
-    right; left; rewrite <- DST1; apply H0.
-    right; right; rewrite <- DST2; apply H0.
-    destruct H0; destruct H0.
-    exists (ZE_Fin x).
-    assert (INV: IA.length_zform (IA.substitute (v, @PureInfinity.conv PureInfinity.Q_ZE (ZE_Fin x)) f) <= n) by solve_le_inv;
-      destruct (IHn _ INV) as [SAT DST].
-    rewrite DST; rewrite <- subst_inf_trans_eq; apply H0.
-    exists ZE_Inf; rewrite DST1; apply H0.
-    exists ZE_NegInf; rewrite DST2; apply H0.
+      assert (INV1: IA.length_zform (IA.substitute(v,Some ZE_Inf)f) <= n) by solve_le_inv; destruct (IHn _ INV1) as [SAT1 DST1];
+      assert (INV2: IA.length_zform(IA.substitute(v,Some ZE_NegInf)f)<=n) by solve_le_inv; destruct (IHn _ INV2) as [SAT2 DST2].
+      destruct q; unfold PureInfinity.QT, IntToInfinity.QT.
+      split; intros; destruct H0 as [x H0]; exists x;
+      assert (INV: IA.length_zform (IA.substitute (v, @IntToInfinity.conv tt x) f) <= n) by solve_le_inv;
+      destruct (IHn _ INV) as [SAT DST];
+      [rewrite subst_inf_trans_eq; rewrite <- DST | rewrite DST; rewrite <- subst_inf_trans_eq]; apply H0.
+      do 2 rewrite I2F.dissatisfied_unfold; split; intros.
+      destruct H0 as [x H0]; destruct x.
+      left; exists z; rewrite subst_inf_trans_eq.
+      assert (INV: IA.length_zform (IA.substitute (v, @PureInfinity.conv PureInfinity.Q_Z z) f) <= n) by solve_le_inv;
+        destruct (IHn _ INV) as [SAT DST].
+      rewrite <- DST; apply H0.
+      right; left; rewrite <- DST1; apply H0.
+      right; right; rewrite <- DST2; apply H0.
+      destruct H0; destruct H0.
+      exists (ZE_Fin x).
+      assert (INV: IA.length_zform (IA.substitute (v, @PureInfinity.conv PureInfinity.Q_ZE (ZE_Fin x)) f) <= n) by solve_le_inv;
+        destruct (IHn _ INV) as [SAT DST].
+      rewrite DST; rewrite <- subst_inf_trans_eq; apply H0.
+      exists ZE_Inf; rewrite DST1; apply H0.
+      exists ZE_NegInf; rewrite DST2; apply H0.
 
-    assert (INV1: IA.length_zform (IA.substitute (v,Some ZE_Inf) f) <= n) by solve_le_inv; destruct (IHn _ INV1) as [SAT1 DST1];
-    assert (INV2: IA.length_zform(IA.substitute(v,Some ZE_NegInf) f)<= n) by solve_le_inv; destruct (IHn _ INV2) as [SAT2 DST2].
-    destruct q; unfold PureInfinity.QT, IntToInfinity.QT.
-    split; intros; assert (INV: IA.length_zform (IA.substitute (v, @IntToInfinity.conv tt x) f) <= n) by solve_le_inv;
-    destruct (IHn _ INV) as [SAT DST];
-    [rewrite subst_inf_trans_eq; rewrite <- DST | rewrite DST; rewrite <- subst_inf_trans_eq]; apply H0.
-    do 2 rewrite I2F.dissatisfied_unfold; split; intros.
-    split; intros.
-    assert (INV: IA.length_zform (IA.substitute (v, @IntToInfinity.conv tt x) f) <= n) by solve_le_inv;
-    destruct (IHn _ INV) as [SAT DST].
-    rewrite subst_inf_trans_eq; rewrite <- DST; apply H0.
-    split; [rewrite <- DST1 | rewrite <- DST2].
-    apply H0. apply H0. destruct H0 as [? [? ?]].
-    destruct x.
-    assert (INV: IA.length_zform (IA.substitute (v, @PureInfinity.conv PureInfinity.Q_Z z) f) <= n) by solve_le_inv;
-      destruct (IHn _ INV) as [SAT DST].
-    rewrite DST; rewrite <- subst_inf_trans_eq; apply H0.
-    rewrite DST1; apply H1. rewrite DST2; apply H2.
-  Qed.
+      assert (INV1: IA.length_zform (IA.substitute(v,Some ZE_Inf)f) <= n) by solve_le_inv; destruct (IHn _ INV1) as [SAT1 DST1];
+      assert (INV2: IA.length_zform(IA.substitute(v,Some ZE_NegInf)f)<=n) by solve_le_inv; destruct (IHn _ INV2) as [SAT2 DST2].
+      destruct q; unfold PureInfinity.QT, IntToInfinity.QT.
+      split; intros; assert (INV: IA.length_zform (IA.substitute (v, @IntToInfinity.conv tt x) f) <= n) by solve_le_inv;
+      destruct (IHn _ INV) as [SAT DST];
+      [rewrite subst_inf_trans_eq; rewrite <- DST | rewrite DST; rewrite <- subst_inf_trans_eq]; apply H0.
+      do 2 rewrite I2F.dissatisfied_unfold; split; intros.
+      split; intros.
+      assert (INV: IA.length_zform (IA.substitute (v, @IntToInfinity.conv tt x) f) <= n) by solve_le_inv;
+        destruct (IHn _ INV) as [SAT DST].
+      rewrite subst_inf_trans_eq; rewrite <- DST; apply H0.
+      split; [rewrite <- DST1 | rewrite <- DST2].
+      apply H0. apply H0. destruct H0 as [? [? ?]].
+      destruct x.
+      assert (INV: IA.length_zform (IA.substitute (v, @PureInfinity.conv PureInfinity.Q_Z z) f) <= n) by solve_le_inv;
+        destruct (IHn _ INV) as [SAT DST].
+      rewrite DST; rewrite <- subst_inf_trans_eq; apply H0.
+      rewrite DST1; apply H1. rewrite DST2; apply H2.
+    Qed.
+
+  End InfinityTransformation.
+
+  Section IntegerTransformation.
+
+    (* Shortened Forms of Boolean Constants *)
+    Definition embed (v : Val) := FA.ZF_BF (FA.ZBF_Const v).
+    Definition FATrue := embed (bool_inj true).
+    Definition FAFalse := embed (bool_inj false).
+    Definition FANone := embed noneVal.
+
+    (* Projection from integers with infinity to integers *)
+    Definition proj (z : IntToInfinity.N.A) : Z :=
+      match z with
+          Some (ZE_Fin x) => x
+        | _ => 0%Z (* This case doesn't happen actually. *)
+      end.
+
+    (* Transform expressions in I2F to FA *)
+    Fixpoint int_trans_exp (exp : I2F.ZExp) : FA.ZExp :=
+      match exp with
+          I2F.ZExp_Var v => FA.ZExp_Var v
+        | I2F.ZExp_Const a => FA.ZExp_Const (proj a)
+        | I2F.ZExp_Add e1 e2 => FA.ZExp_Add (int_trans_exp e1) (int_trans_exp e2)
+        | I2F.ZExp_Inv e => FA.ZExp_Inv (int_trans_exp e)
+        | I2F.ZExp_Sub e1 e2 => FA.ZExp_Sub (int_trans_exp e1) (int_trans_exp e2)
+        | I2F.ZExp_Mult z e => FA.ZExp_Mult z (int_trans_exp e)
+      end.
+
+    (* Transform boolean forms in I2F to FA *)
+    Definition int_trans_bf (bf : I2F.ZBF) : FA.ZF :=
+      match bf with
+          I2F.ZBF_Const f => FA.ZF_BF (FA.ZBF_Const f)
+        | I2F.ZBF_Lt e1 e2 =>
+          match (I2F.dexp2ZE e1), (I2F.dexp2ZE e2) with
+              None, _
+            | _, None => FANone
+            | Some ZE_NegInf, Some x => if ZE_eq_dec x ZE_NegInf then FAFalse else FATrue
+            | Some x, Some ZE_Inf => if ZE_eq_dec x ZE_Inf then FAFalse else FATrue
+            | Some _, Some ZE_NegInf => FAFalse
+            | Some ZE_Inf, Some _ => FAFalse
+            | Some (ZE_Fin _), Some (ZE_Fin _) => FA.ZF_BF (FA.ZBF_Lt (int_trans_exp e1) (int_trans_exp e2))
+          end
+        | I2F.ZBF_Lte e1 e2 =>
+          match (I2F.dexp2ZE e1), (I2F.dexp2ZE e2) with
+              None, _
+            | _, None => FANone
+            | Some _, Some ZE_Inf => FATrue
+            | Some ZE_NegInf, Some _ => FATrue
+            | Some ZE_Inf, Some x => if ZE_eq_dec x ZE_Inf then FATrue else FAFalse
+            | Some x, Some ZE_NegInf => if ZE_eq_dec x ZE_NegInf then FATrue else FAFalse
+            | Some (ZE_Fin _), Some (ZE_Fin _) => FA.ZF_BF (FA.ZBF_Lte (int_trans_exp e1) (int_trans_exp e2))
+          end
+        | I2F.ZBF_Gt e1 e2 =>
+          match (I2F.dexp2ZE e1), (I2F.dexp2ZE e2) with
+              None, _
+            | _, None => FANone
+            | Some ZE_Inf, Some x => if ZE_eq_dec x ZE_Inf then FAFalse else FATrue
+            | Some x, Some ZE_NegInf => if ZE_eq_dec x ZE_NegInf then FAFalse else FATrue
+            | Some _, Some ZE_Inf => FAFalse
+            | Some ZE_NegInf, Some _ => FAFalse
+            | Some (ZE_Fin _), Some (ZE_Fin _) => FA.ZF_BF (FA.ZBF_Gt (int_trans_exp e1) (int_trans_exp e2))
+          end
+        | I2F.ZBF_Gte e1 e2 =>
+          match (I2F.dexp2ZE e1), (I2F.dexp2ZE e2) with
+              None, _
+            | _, None => FANone
+            | Some _, Some ZE_NegInf => FATrue
+            | Some ZE_Inf, Some _ => FATrue
+            | Some ZE_NegInf, Some x => if ZE_eq_dec x ZE_NegInf then FATrue else FAFalse
+            | Some x, Some ZE_Inf => if ZE_eq_dec x ZE_Inf then FATrue else FAFalse
+            | Some (ZE_Fin _), Some (ZE_Fin _) => FA.ZF_BF (FA.ZBF_Gte (int_trans_exp e1) (int_trans_exp e2))
+          end
+        | I2F.ZBF_Eq e1 e2 =>
+          match (I2F.dexp2ZE e1), (I2F.dexp2ZE e2) with
+              None, _
+            | _, None => FANone
+            | Some ZE_NegInf, Some x
+            | Some x, Some ZE_NegInf => if ZE_eq_dec x ZE_NegInf then FATrue else FAFalse
+            | Some ZE_Inf, Some x
+            | Some x, Some ZE_Inf => if ZE_eq_dec x ZE_Inf then FATrue else FAFalse
+            | Some (ZE_Fin _), Some (ZE_Fin _) => FA.ZF_BF (FA.ZBF_Eq (int_trans_exp e1) (int_trans_exp e2))
+          end
+        | I2F.ZBF_Eq_Max e1 e2 e3 =>
+          match (I2F.dexp2ZE e1), (I2F.dexp2ZE e2), (I2F.dexp2ZE e3) with
+              None, _, _
+            | _, None, _
+            | _, _, None => FANone
+            | Some ZE_NegInf, Some x, Some y =>
+              if (ZE_eq_dec x ZE_NegInf)
+              then if (ZE_eq_dec y ZE_NegInf)
+                   then FATrue
+                   else FAFalse
+              else FAFalse
+            | Some ZE_Inf, Some x, Some y =>
+              if ZE_eq_dec x ZE_Inf
+              then FATrue
+              else if ZE_eq_dec y ZE_Inf
+                   then FATrue
+                   else FAFalse
+            | Some (ZE_Fin _), Some ZE_NegInf, Some y =>
+              match y with
+                  ZE_NegInf
+                | ZE_Inf => FAFalse
+                | _ => FA.ZF_BF (FA.ZBF_Eq (int_trans_exp e1) (int_trans_exp e3))
+              end
+            | Some (ZE_Fin _), Some y, Some ZE_NegInf =>
+              match y with
+                  ZE_NegInf
+                | ZE_Inf => FAFalse
+                | _ => FA.ZF_BF (FA.ZBF_Eq (int_trans_exp e1) (int_trans_exp e2))
+              end
+            | Some (ZE_Fin _), Some ZE_Inf, Some y
+            | Some (ZE_Fin _), Some y, Some ZE_Inf => FAFalse
+            | Some (ZE_Fin _), Some (ZE_Fin _), Some(ZE_Fin _) =>
+              FA.ZF_BF (FA.ZBF_Eq_Max (int_trans_exp e1) (int_trans_exp e2) (int_trans_exp e3))
+          end
+        | I2F.ZBF_Eq_Min e1 e2 e3 =>
+          match (I2F.dexp2ZE e1), (I2F.dexp2ZE e2), (I2F.dexp2ZE e3) with
+              None, _, _
+            | _, None, _
+            | _, _, None => FANone
+            | Some ZE_NegInf, Some x, Some y =>
+              if ZE_eq_dec x ZE_NegInf
+              then FATrue
+              else if ZE_eq_dec y ZE_NegInf
+                   then FATrue
+                   else FAFalse
+            | Some ZE_Inf, Some x, Some y =>
+              if (ZE_eq_dec x ZE_Inf)
+              then if (ZE_eq_dec y ZE_Inf)
+                   then FATrue
+                   else FAFalse
+              else FAFalse
+            | Some (ZE_Fin _), Some ZE_NegInf, Some y
+            | Some (ZE_Fin _), Some y, Some ZE_NegInf => FAFalse
+            | Some (ZE_Fin _), Some ZE_Inf, Some y =>
+              match y with
+                  ZE_Inf
+                | ZE_NegInf => FAFalse
+                | _ => FA.ZF_BF (FA.ZBF_Eq (int_trans_exp e1) (int_trans_exp e3))
+              end
+            | Some (ZE_Fin _), Some y, Some ZE_Inf =>
+              match y with
+                  ZE_Inf
+                | ZE_NegInf => FAFalse
+                | _ => FA.ZF_BF (FA.ZBF_Eq (int_trans_exp e1) (int_trans_exp e2))
+              end
+            | Some (ZE_Fin _), Some (ZE_Fin _), Some(ZE_Fin _) =>
+              FA.ZF_BF (FA.ZBF_Eq_Min (int_trans_exp e1) (int_trans_exp e2) (int_trans_exp e3))
+          end
+        | I2F.ZBF_Neq e1 e2 =>
+          match (I2F.dexp2ZE e1), (I2F.dexp2ZE e2) with
+              None, _
+            | _, None => embed (truth_not noneVal)
+            | Some ZE_NegInf, Some x
+            | Some x, Some ZE_NegInf => if ZE_eq_dec x ZE_NegInf then FAFalse else FATrue
+            | Some ZE_Inf, Some x
+            | Some x, Some ZE_Inf => if ZE_eq_dec x ZE_Inf then FAFalse else FATrue
+            | Some (ZE_Fin _), Some (ZE_Fin _) => FA.ZF_BF (FA.ZBF_Neq (int_trans_exp e1) (int_trans_exp e2))
+          end
+      end.
+
+    (* If natural number product is finite, then either the constant is zero or the variable is finite. *)
+    Lemma nat_nummult_finite: forall c v x,
+                                I2F.num_mult_nat c v = Some (IntToInfinity.N.ZE_Fin x)
+                                -> ((c = 0 /\ x = 0%Z) \/ (exists n, v = Some (ZE_Fin n) /\ FA.num_mult_nat c n = x)).
+    Proof.
+      induction c; simpl; intros.
+      left; split; auto; injection H; auto.
+      apply numplus_finite in H.
+      destruct H, H, H.
+      destruct H0.
+      right; exists x0.
+      split; auto.
+      apply IHc in H0.
+      destruct H0, H0.
+      rewrite H0.
+      rewrite H2 in H1.
+      simpl; auto.
+      destruct H0.
+      assert (x2 = x0).
+      rewrite H in H0.
+      injection H0; auto.
+      rewrite H3 in H2.
+      rewrite H2; auto.
+    Qed.
+
+    (* If integer product is finite, then either the constant is zero or the variable is finite. *)
+    Lemma nummult_finite: forall c v x, I2F.num_mult c v = Some (IntToInfinity.N.ZE_Fin x)
+                                        -> (c = 0%Z /\ x = 0%Z) \/
+                                           (exists n, v = Some (ZE_Fin n) /\ FA.num_mult c n = x).
+    Proof.
+      destruct c; simpl; intros.
+      left; split; auto; injection H; auto.
+      apply nat_nummult_finite in H.
+      destruct H.
+      destruct H.
+      left.
+      assert (0 < Pos.to_nat p) by apply Pos2Nat.is_pos.
+      omega.
+      destruct H, H.
+      right; exists x0.
+      split; auto.
+      apply numneg_finite in H.
+      destruct H, H.
+      apply nat_nummult_finite in H.
+      destruct H.
+      assert (0 < Pos.to_nat p) by apply Pos2Nat.is_pos.
+      omega.
+      destruct H, H.
+      right; exists x1.
+      split; auto.
+      rewrite H1; auto.
+    Qed.
+
+    (* Expression transform from I2F to FA keeps the finiteness. *)
+    Lemma dexp2ZE_int_trans_eq: forall z x, I2F.dexp2ZE z = Some (IntToInfinity.N.ZE_Fin x) -> FA.dexp2ZE (int_trans_exp z) = x.
+    Proof.
+      induction z; simpl; intros.
+      injection H; auto.
+      rewrite H; auto.
+      apply numplus_finite in H;
+        destruct H, H, H; destruct H0;
+        apply IHz1 in H;
+        apply IHz2 in H0;
+        rewrite H, H0; auto.
+
+      apply numneg_finite in H;
+        destruct H, H;
+        apply IHz in H;
+        rewrite H; auto.
+
+      apply numplus_finite in H;
+        destruct H, H, H; destruct H0;
+        apply numneg_finite in H0;
+        destruct H0, H0;
+        apply IHz1 in H;
+        apply IHz2 in H0;
+        rewrite H, H0;
+        rewrite <- H2 in H1;
+        auto.
+
+      apply nummult_finite in H.
+      destruct H, H.
+      rewrite H, H0.
+      simpl; auto.
+      destruct H.
+      apply IHz in H.
+      rewrite H; auto.
+    Qed.
+
+    Ltac smash_int_trans_bf :=
+      repeat match goal with
+               | [|- context[FinRel.num_leq _ _]] => unfold FinRel.num_leq
+               | [ H: FANone = _ |- _] => unfold FANone in H; unfold embed in H; inversion H; simpl
+               | [|- context[truth_not (bool_inj false)]] => rewrite tautology_1
+               | [|- context[truth_not (bool_inj true)]] => rewrite tautology_2
+               | [|- context[truth_and ?X ?X]] => rewrite tautology_3
+               | [|- context[truth_and (bool_inj true) (bool_inj false)]] => rewrite tautology_4
+               | [|- context[truth_and (bool_inj false) (bool_inj true)]] => rewrite tautology_5
+               | [|- context[truth_or ?X ?X]] => rewrite tautology_6
+               | [|- context[truth_or (bool_inj true) (bool_inj false)]] => rewrite tautology_7
+               | [|- context[truth_or (bool_inj false) (bool_inj true)]] => rewrite tautology_8
+               | [|- context[truth_and noneVal (truth_not noneVal)]] => rewrite none_tautology_1
+               | [|- context[truth_and noneVal (bool_inj true)]] => rewrite none_tautology_2
+               | [|- context[truth_and noneVal (bool_inj false)]] => rewrite none_tautology_3
+               | [|- context[truth_or noneVal (bool_inj false)]] => rewrite none_tautology_4
+               | [|- context[truth_or (bool_inj false) noneVal]] => rewrite none_tautology_5
+               | [H: I2F.dexp2ZE ?z = Some (IntToInfinity.N.ZE_Fin ?x) |- context[FA.dexp2ZE (int_trans_exp ?z)]]
+                 => rewrite (dexp2ZE_int_trans_eq z x)
+               | [|- ?X <-> ?X] => tauto
+               | [H: ?X |- ?X] => apply H
+               | [|- context[match (I2F.dexp2ZE ?X) with _ => _ end]] => destruct (I2F.dexp2ZE X) eqn: ?; simpl
+               | [|- context[match ?X with _ => _ end]] => destruct X eqn: ?; simpl
+               | [H: context[match ?X with _ => _ end] |- _] => destruct X eqn: ?; simpl
+               | [|- context[InfRel.num_leq _ _]] => unfold InfRel.num_leq
+               | [_: (?a <= ?b)%Z, _: ~ (?a <= ?b)%Z |- _] => contradiction
+               | [_: ~ (?a <= ?b)%Z, _: ~ (?b <= ?a)%Z |- _] => exfalso; intuition
+               | [|- context[truth_and (bool_inj true) noneVal]] => rewrite truth_and_comm, none_tautology_2
+               | [|- context[truth_and (bool_inj false) noneVal]] => rewrite truth_and_comm, none_tautology_3
+             end.
+
+    (* Boolean transformation from I2F to FA keeps the validity. *)
+    Lemma int_trans_bf_sat: forall bf, I2F.satisfied (I2F.ZF_BF bf) <-> FA.satisfied (int_trans_bf bf).
+    Proof. destruct bf; simpl; rewrite I2F.satisfied_unfold, FA.satisfied_unfold; simpl; smash_int_trans_bf. Qed.
+
+    Lemma int_trans_bf_dst: forall bf, I2F.dissatisfied (I2F.ZF_BF bf) <-> FA.dissatisfied (int_trans_bf bf).
+    Proof. destruct bf; simpl; rewrite I2F.dissatisfied_unfold, FA.dissatisfied_unfold; simpl; smash_int_trans_bf. Qed.
+
+  End IntegerTransformation.
 
 End InfSolver.
